theories/examples/mem_trans_msg_send/proof.v
@@ -144,7 +144,7 @@ Program Definition zero : Imm := I (finz.FinZ 0 _ _) _.
 Program Definition one : Imm := I (finz.FinZ 1 _ _) _.
 Program Definition two : Imm := I (finz.FinZ 2 _ _) _.
 Program Definition four : Imm := I (finz.FinZ 4 _ _) _.
-Program Definition mem_descriptor_length : Imm := I (finz.FinZ 6 _ _) _.
+Program Definition mem_descriptor_length : Imm := I (finz.FinZ 5 _ _) _.
 
 Section proof.
 
@@ -174,7 +174,7 @@ Section proof.
       mov_word_I R4 addr;
       str_I R4 R5;
       (* Lend page *)
-      mov_word_I R0 mem_lend_I;
+      mov_word_I R0 mem_share_I;
       mov_word_I R1 mem_descriptor_length;
       hvc_I;
       (* Send handle *)
@@ -189,10 +189,10 @@ Section proof.
       mov_word_I R0 run_I;
       mov_word_I R1 (encode_vmid V1);
       hvc_I;
-      (* Reclaim page *)
-      mov_word_I R0 mem_reclaim_I;
-      mov_reg_I R1 R3;
-      hvc_I;
+      (* (* Reclaim page *) *)
+      (* mov_word_I R0 mem_reclaim_I; *)
+      (* mov_reg_I R1 R3; *)
+      (* hvc_I; *)
       (* Run VM 2 (unknown vm *)
       mov_word_I R0 run_I;
       mov_word_I R1 (encode_vmid V2);
@@ -217,10 +217,10 @@ Section proof.
       mov_word_I R3 four;
       mov_word_I R5 addr;
       str_I R3 R5;
-      (* Relinquish page *)
-      mov_word_I R0 mem_relinquish_I;
-      mov_reg_I R1 R4;
-      hvc_I;
+      (* (* Relinquish page *) *)
+      (* mov_word_I R0 mem_relinquish_I; *)
+      (* mov_reg_I R1 R4; *)
+      (* hvc_I; *)
       (* Yield back *)
       mov_word_I R0 yield_I;
       hvc_I
@@ -240,12 +240,14 @@ Section proof.
     let RX1 := (RX_state@V1 := None ∗ mailbox.rx_page V1 p_rx1 ∗ ∃ mem_rx, memory_page p_rx1 mem_rx)%I in
     let RX2 := (RX_state@V2 := None ∗ mailbox.rx_page V2 p_rx2 ∗ ∃ mem_rx, memory_page p_rx2 mem_rx)%I in
     let program0 := rywu_program0 addr p_tx0imm in
+    of_pid (tpa addr) = addr ->
     (* Disjoint pages *)
     (of_pid p_tx0 = p_tx0imm) ->
     (of_pid p_pg0 = p_pg0imm) ->
     (p_pg0 ∉ ({[(tpa addr); p_tx0; p_pg2; p_tx2; p_rx2]}:gset _)) ->
     tpa addr ≠ p_rx0 ->
     tpa addr ≠ p_pg0 ->
+    tpa addr ≠ p_tx0 ->
     p_tx0 ≠ p_rx0 ->
     (* Addresses-values connection *)
     seq_in_page (of_pid p_pg0) (length program0) p_pg0 ->
@@ -297,16 +299,16 @@ Section proof.
                  )}}%I.
   Proof.
     rewrite /vmprop_unknown.
-    iIntros (Htxeq Hpgeq HnIn_p HneAddr_RX0 HneAddr_PG0 HneTX0_RX0 HIn) "((p_1 & p_2 & p_3 & p_4 & p_5 & p_6 & p_7 
+    iIntros (Haddr Htxeq Hpgeq HnIn_p HneAddr_RX0 HneAddr_PG0 HneAddr_TX0 HneTX0_RX0 HIn) "((p_1 & p_2 & p_3 & p_4 & p_5 & p_6 & p_7 
             & p_8 & p_9 & p_10 & p_11 & p_12 & p_13 & p_14 & p_15 & p_16 
             & p_17 & p_18 & p_19 & p_20 & p_21 & p_22 & p_23 & p_24 & p_25
             & p_26 & p_27 & p_28 & p_29 & p_30 & p_31 & p_32 & p_33 & p_34
-            & p_35 & p_36 & p_37 & p_38 & p_39 & _) 
+            & p_35 & p_36 & _) 
          & (%memv & mem) & (%txmemgm & txmem) & OE & acc & tx & PCz & (%r0 & R0z) & (%r1 & R1z) & (%r2 & R2z) 
          & (%r3 & R3z) & (%r4 & R4z) & (%r5 & R5z) 
          & prop0 & prop1 & prop2 & acc2 & LB_auth & hp & (RX0st & (RX0page & RX0own & RX0excl) & RX0mem) 
-         & (RX1st & (RX1page & RX1own & RX1excl) & RX1mem) & (RX2st & (RX2page & RX2own & RX2excl) & RX2mem))".
-    pose proof (seq_in_page_forall2 _ _ _ HIn) as Hforall.
+         & (RX1st & (RX1page & RX1own & RX1excl) & RX1mem) & (RX2st & (RX2page & RX2own & RX2excl) & RX2mem))". 
+   pose proof (seq_in_page_forall2 _ _ _ HIn) as Hforall.
     fold_finz_plus_one.
     repeat (rewrite finz_succN_correct).
     (* iEval (rewrite finz_succN_one) in "p_2". *)
@@ -770,14 +772,6 @@ Section proof.
     apply elem_of_singleton_2.
     reflexivity.
     apply finz_succN_in_seq; simpl; lia.
-    simpl.
-    TODO: bug
-  Abort.
-    cbn in domtxmem.
-    simpl in domtxmem.
-    clear HnIn_p domtxmem.
-    (* clear -HnIn_p HIn Hnottx. *)
-    auto.
     rewrite HIn.
     rewrite to_pid_aligned_eq.
     assumption.
@@ -790,41 +784,50 @@ Section proof.
     iIntros "(PCz & _ & R5z & txmem1 & R4z & acc & tx & RX0page) _".
     (* add_I R5 R3 *)
     rewrite wp_sswp.
-    iApply ((@add _ _ _ _ _ _ (add_I R5 R3) p_tx0imm one 1%Qp (tpa p_tx0) (((((((p_pg0 ^+ 1) ^+ 1) ^+ 1) ^+ 1) ^+ 1) ^+ 1) ^+ 1)%f R5 R3 ({[tpa addr]} ∪ {[p_pg0; tpa p_tx0]})) with "[p_8 PCz acc R5z R3z tx]").
+    iEval (rewrite finz_plus_one_simpl) in "PCz".
+    rewrite Z_of_nat_simpl.
+    iEval (simpl) in "PCz".
+    iApply ((@add _ _ _ _ _ _ (add_I R5 R3) p_tx0imm one 1%Qp (tpa p_tx0) (p_pg0 ^+ 7%nat)%f R5 R3 ({[tpa addr]} ∪ {[p_pg0; tpa p_tx0]})) with "[p_8 PCz acc R5z R3z tx]").
     apply decode_encode_instruction.
     apply elem_of_union_r.
     apply elem_of_union_l.
     apply elem_of_singleton_2.
     rewrite HIn.
     reflexivity.
-    set_solver +.
+    apply finz_succN_in_seq; simpl; lia.
     rewrite HIn.
     rewrite to_pid_aligned_eq.
     assumption.
-    set_solver +.
+    apply finz_succN_in_seq; simpl; lia.
     iFrame.    
     iModIntro.
     iIntros "(PCz & _ & R5z & R3z & acc & tx) _".
     (* mov_word_I R4 zero *)
     rewrite wp_sswp.
-    iApply ((@mov_word _ _ _ _ _ _ _ _ _ ({[tpa addr]} ∪ {[p_pg0; tpa p_tx0]}) (tpa p_tx0) ((((((((p_pg0 ^+ 1) ^+ 1) ^+ 1) ^+ 1) ^+ 1) ^+ 1) ^+ 1) ^+ 1)%f zero R4) with "[p_9 PCz acc tx R4z]").
+    iEval (rewrite finz_plus_one_simpl) in "PCz".
+    rewrite Z_of_nat_simpl.
+    iEval (simpl) in "PCz".
+    iApply ((@mov_word _ _ _ _ _ _ _ _ _ ({[tpa addr]} ∪ {[p_pg0; tpa p_tx0]}) (tpa p_tx0) (p_pg0 ^+ 8%nat)%f zero R4) with "[p_9 PCz acc tx R4z]").
     apply decode_encode_instruction.
     apply elem_of_union_r.
     apply elem_of_union_l.
     apply elem_of_singleton_2.
     rewrite HIn.
     reflexivity.
-    set_solver +.    
+    apply finz_succN_in_seq; simpl; lia.
     rewrite HIn.
     rewrite to_pid_aligned_eq.
     assumption.
-    set_solver +.
+    apply finz_succN_in_seq; simpl; lia.
     iFrame.
     iModIntro.
     iIntros "(PCz & _ & acc & tx & R4z) _".
     (* str_I R4 R5 *)
     rewrite wp_sswp.
-    iApply ((@str _ _ _ _ _ _ _ zero w2 1%Qp p_rx0 (tpa p_tx0) ({[tpa addr]} ∪ {[p_pg0; tpa p_tx0]}) (((((((((p_pg0 ^+ 1) ^+ 1) ^+ 1) ^+ 1) ^+ 1) ^+ 1) ^+ 1) ^+ 1) ^+ 1)%f (p_tx0 ^+ 1)%f R4 R5) with "[p_10 PCz acc txmem2 RX0page tx R4z R5z]").
+    iEval (rewrite finz_plus_one_simpl) in "PCz".
+    rewrite Z_of_nat_simpl.
+    iEval (simpl) in "PCz".
+    iApply ((@str _ _ _ _ _ _ _ zero w2 1%Qp p_rx0 (tpa p_tx0) ({[tpa addr]} ∪ {[p_pg0; tpa p_tx0]}) (p_pg0 ^+ 9%nat)%f (p_tx0 ^+ 1)%f R4 R5) with "[p_10 PCz acc txmem2 RX0page tx R4z R5z]").
     apply decode_encode_instruction.
     apply union_subseteq_r'.
     apply union_least.
@@ -833,753 +836,1378 @@ Section proof.
     apply elem_of_singleton_2.
     {
       rewrite to_pid_aligned_eq.
-      apply to_pid_aligned_in_page.
-      unfold addr_in_page.
-      split.
-      apply Is_true_true_2.
-      solve_finz.
-      apply Is_true_true_2.
-      solve_finz.
+      rewrite (finz_succN_pid' p_tx0 1).
+      reflexivity.
+      lia.
     }
     rewrite singleton_subseteq_l.
     apply elem_of_union_l.
     apply elem_of_singleton_2.
     apply HIn.
-    set_solver +.
+    apply finz_succN_in_seq; simpl; lia.
     rewrite HIn.
     rewrite to_pid_aligned_eq.
     assumption.
-    set_solver +.
-    assert (tpa (p_tx0 ^+ 1)%f = p_tx0) as ->.
-    {
-      apply to_pid_aligned_in_page.
-      unfold addr_in_page.
-      split.
-      apply Is_true_true_2.
-      solve_finz.
-      apply Is_true_true_2.
-      solve_finz.
-    }
+    apply finz_succN_in_seq; simpl; lia.
+    rewrite (finz_succN_pid' p_tx0 1).
     assumption.
+    lia.
     rewrite Htxeq.
     iFrame.
     iModIntro.
     iIntros "(PCz & _ & R5z & txmem2 & R4z & acc & tx & RX0page) _".
     (* add_I R5 R3 *)
     rewrite wp_sswp.
+    iEval (rewrite finz_plus_one_simpl) in "PCz".
+    rewrite Z_of_nat_simpl.
+    iEval (simpl) in "PCz".
     iApply (@add _ _ _ _ _ _ (add_I R5 R3) (p_tx0imm ^+ 1)%f one 1%Qp (tpa p_tx0)
-              ((((((((((p_pg0 ^+ 1) ^+ 1) ^+ 1) ^+ 1) ^+ 1) ^+ 1) ^+ 1) ^+ 1) ^+ 1) ^+ 1)%f
+              (p_pg0 ^+ 10%nat)%f
               R5 R3 ({[tpa addr]} ∪ {[p_pg0; tpa p_tx0]}) with "[p_11 PCz acc R5z R3z tx]").
     apply decode_encode_instruction. 
     apply elem_of_union_r.
     apply elem_of_union_l.
     apply elem_of_singleton_2.
-    {
-      apply to_pid_aligned_in_page.
-      unfold addr_in_page.
-      split.
-      apply Is_true_true_2.
-      solve_finz.
-      apply Is_true_true_2.
-      solve_finz.
-    }
+    rewrite (finz_succN_pid' p_pg0 10).
+    reflexivity.
+    lia.
     rewrite HIn.
     rewrite to_pid_aligned_eq.
     assumption.
-    set_solver +.
+    apply finz_succN_in_seq; simpl; lia.
     rewrite Htxeq.
     iFrame.
     iModIntro.
     iIntros "(PCz & _ & R5z & R3z & acc & tx) _".
     (* (* mov_word_I R4 one *) *)
     rewrite wp_sswp.
+    iEval (rewrite finz_plus_one_simpl) in "PCz".
+    rewrite Z_of_nat_simpl.
+    iEval (simpl) in "PCz".
     iApply ((@mov_word _ _ _ _ _ _ _ _ _ ({[tpa addr]} ∪ {[p_pg0; tpa p_tx0]}) (tpa p_tx0)
-               (((((((((((p_pg0 ^+ 1) ^+ 1) ^+ 1) ^+ 1) ^+ 1) ^+ 1) ^+ 1) ^+ 1) ^+ 1) ^+ 1) ^+ 1)%f
+               (p_pg0 ^+ 11%nat)%f
                one R4) with "[p_12 PCz acc tx R4z]").
     apply decode_encode_instruction.
     apply elem_of_union_r.
     apply elem_of_union_l.
     apply elem_of_singleton_2.
-    {
-      apply to_pid_aligned_in_page.
-      unfold addr_in_page.
-      split.
-      apply Is_true_true_2.
-      solve_finz.
-      apply Is_true_true_2.
-      solve_finz.
-    }
+    rewrite (finz_succN_pid' p_pg0 11).
+    reflexivity.
+    lia.
     rewrite HIn.
     rewrite to_pid_aligned_eq.
     assumption.
-    set_solver +.
+    apply finz_succN_in_seq; simpl; lia.
+    rewrite Htxeq.
+    iFrame.
+    iModIntro.
+    iIntros "(PCz & _ & acc & tx & R4z) _".
+    rewrite wp_sswp.
+    iEval (rewrite finz_plus_one_simpl) in "PCz".
+    rewrite Z_of_nat_simpl.
+    iEval (simpl) in "PCz".
+    iApply ((@str _ _ _ _ _ _ _ one w3 1%Qp p_rx0 (tpa p_tx0) ({[tpa addr]} ∪ {[p_pg0; tpa p_tx0]}) (p_pg0 ^+ 12%nat)%f ((p_tx0 ^+ 1) ^+ 1)%f R4 R5) with "[p_13 PCz acc txmem3 RX0page tx R4z R5z]").
+    apply decode_encode_instruction.
+    apply union_subseteq_r'.
+    apply union_least.
+    rewrite singleton_subseteq_l.    
+    apply elem_of_union_r.
+    apply elem_of_singleton_2.
+    {
+      rewrite to_pid_aligned_eq.
+      repeat (rewrite finz_succN_one).
+      repeat (rewrite finz_succN_idemp).
+      simpl.
+      rewrite finz_succN_correct.
+      rewrite (finz_succN_pid' p_tx0 2).
+      reflexivity.
+      lia.
+    }
+    rewrite singleton_subseteq_l.
+    apply elem_of_union_l.
+    apply elem_of_singleton_2.
+    apply HIn.
+    apply finz_succN_in_seq; simpl; lia.
+    rewrite HIn.
+    rewrite to_pid_aligned_eq.
+    assumption.
+    apply finz_succN_in_seq; simpl; lia.
+    repeat (rewrite finz_succN_one).
+    repeat (rewrite finz_succN_idemp).
+    simpl.
+    rewrite finz_succN_correct.
+    rewrite (finz_succN_pid' p_tx0 2).
+    assumption.
+    lia.
+    rewrite Htxeq.
+    iFrame.
+    iModIntro.
+    iIntros "(PCz & _ & R5z & txmem3 & R4z & acc & tx & RX0page) _".
+    (* add_I R5 R3 *)
+    rewrite wp_sswp.
+    iEval (rewrite finz_plus_one_simpl) in "PCz".
+    rewrite Z_of_nat_simpl.
+    iEval (simpl) in "PCz".
+    iApply (@add _ _ _ _ _ _ (add_I R5 R3) ((p_tx0imm ^+ 1) ^+ 1)%f one 1%Qp (tpa p_tx0)
+              (p_pg0 ^+ 13%nat)%f
+              R5 R3 ({[tpa addr]} ∪ {[p_pg0; tpa p_tx0]}) with "[p_14 PCz acc R5z R3z tx]").
+    apply decode_encode_instruction. 
+    apply elem_of_union_r.
+    apply elem_of_union_l.
+    apply elem_of_singleton_2.
+    rewrite (finz_succN_pid' p_pg0 13).
+    reflexivity.
+    lia.
+    rewrite HIn.
+    rewrite to_pid_aligned_eq.
+    assumption.
+    apply finz_succN_in_seq; simpl; lia.
     rewrite Htxeq.
     iFrame.
     iModIntro.
     iIntros "(PCz & _ & R5z & R3z & acc & tx) _".
-    (* iApply ((mov_word _ one R4) with "[p_12 PCz acc tx R4z]"); iFrameAutoSolve. *)
-    (* rewrite HIn. *)
-    (* set_solver +. *)
-    (* set_solver +. *)
-    (* rewrite HIn. *)
-    (* assumption. *)
-    (* set_solver +. *)
-    (* iModIntro. *)
-    (* iIntros "(PCz & _ & acc & tx & R4z) _". *)
-    (* (* str_I R4 R5 *) *)
-    (* rewrite wp_sswp. *)
-    (* iDestruct "txmem" as "(txmem3 & txmem)". *)
-    (* iApply ((str _ ((p_tx0 ^+ 1) ^+ 1)%f R4 R5) with "[p_13 PCz acc txmem3 RX0page tx R4z R5z]"); iFrameAutoSolve. *)
-    (* (* solvable *) *)
-    (* admit. *)
-    (* rewrite HIn. *)
-    (* assumption. *)
-    (* set_solver +. *)
-    (* assert (tpa ((p_tx0 ^+ 1) ^+ 1)%f = tpa p_tx0) as ->. *)
-    (* admit. *)
-    (* assert (tpa p_tx0 ≠ p_rx0) as temp. *)
-    (* admit. *)
-    (* exact temp. *)
-    (* iModIntro. *)
-    (* iIntros "(PCz & _ & R5z & txmem3 & R4z & acc & tx & RX0page) _". *)
-    (* (* add_I R5 R3 *) *)
-    (* rewrite wp_sswp. *)
-    (* iApply ((add _ R5 R3 _) with "[p_14 PCz acc R5z R3z tx]"); iFrameAutoSolve. *)
-    (* apply elem_of_union_r. *)
-    (* apply elem_of_union_l. *)
-    (* apply elem_of_singleton_2. *)
-    (* rewrite HIn. *)
-    (* reflexivity. *)
-    (* set_solver +. *)
-    (* rewrite HIn. *)
-    (* assumption. *)
-    (* set_solver +. *)
-    (* iModIntro. *)
-    (* iIntros "(PCz & _ & R5z & R3z & acc & tx) _". *)
-    (* (* mov_word_I R4 (encode_vmid V1) *) *)
-    (* rewrite wp_sswp. *)
-    (* iApply ((mov_word _ (encode_vmid V1) R4) with "[p_15 PCz acc tx R4z]"); iFrameAutoSolve. *)
-    (* rewrite HIn. *)
-    (* set_solver +. *)
-    (* set_solver +. *)
-    (* rewrite HIn. *)
-    (* assumption. *)
-    (* set_solver +. *)
-    (* iModIntro. *)
-    (* iIntros "(PCz & _ & acc & tx & R4z) _". *)
-    (* (* str_I R4 R5 *) *)
-    (* rewrite wp_sswp. *)
-    (* iDestruct "txmem" as "(txmem4 & txmem)". *)
-    (* iApply ((str _ (((p_tx0 ^+ 1) ^+ 1) ^+ 1)%f R4 R5) with "[p_16 PCz acc txmem4 RX0page tx R4z R5z]"); iFrameAutoSolve. *)
-    (* (* solvable *) *)
-    (* admit. *)
-    (* rewrite HIn. *)
-    (* assumption. *)
-    (* set_solver +. *)
-    (* assert (tpa (((p_tx0 ^+ 1) ^+ 1) ^+ 1)%f = tpa p_tx0) as ->. *)
-    (* admit. *)
-    (* assert (tpa p_tx0 ≠ p_rx0) as temp. *)
-    (* admit. *)
-    (* exact temp. *)
-    (* iModIntro. *)
-    (* iIntros "(PCz & _ & R5z & txmem4 & R4z & acc & tx & RX0page) _". *)
-    (* (* add_I R5 R3 *) *)
-    (* rewrite wp_sswp. *)
-    (* iApply ((add _ R5 R3 _) with "[p_17 PCz acc R5z R3z tx]"); iFrameAutoSolve. *)
-    (* apply elem_of_union_r. *)
-    (* apply elem_of_union_l. *)
-    (* apply elem_of_singleton_2. *)
-    (* rewrite HIn. *)
-    (* reflexivity. *)
-    (* set_solver +. *)
-    (* rewrite HIn. *)
-    (* assumption. *)
-    (* set_solver +. *)
-    (* iModIntro. *)
-    (* iIntros "(PCz & _ & R5z & R3z & acc & tx) _". *)
-    (* (* mov_word_I R4 addr *) *)
-    (* rewrite wp_sswp. *)
-    (* iApply ((mov_word _ addr R4) with "[p_18 PCz acc tx R4z]"); iFrameAutoSolve. *)
-    (* rewrite HIn. *)
-    (* set_solver +. *)
-    (* set_solver +. *)
-    (* rewrite HIn. *)
-    (* assumption. *)
-    (* set_solver +. *)
-    (* iModIntro. *)
-    (* iIntros "(PCz & _ & acc & tx & R4z) _". *)
-    (* (* str_I R4 R5 *) *)
-    (* rewrite wp_sswp. *)
-    (* iDestruct "txmem" as "(txmem5 & _)". *)
-    (* iApply ((str _ ((((p_tx0 ^+ 1) ^+ 1) ^+ 1) ^+ 1)%f R4 R5) with "[p_19 PCz acc txmem5 RX0page tx R4z R5z]"); iFrameAutoSolve. *)
-    (* (* solvable *) *)
-    (* admit. *)
-    (* rewrite HIn. *)
-    (* assumption. *)
-    (* set_solver +. *)
-    (* assert (tpa ((((p_tx0 ^+ 1) ^+ 1) ^+ 1) ^+ 1)%f = tpa p_tx0) as ->. *)
-    (* admit. *)
-    (* assert (tpa p_tx0 ≠ p_rx0) as temp. *)
-    (* admit. *)
-    (* exact temp. *)
-    (* iModIntro. *)
-    (* iIntros "(PCz & _ & R5z & txmem5 & R4z & acc & tx & RX0page) _". *)
-    (* (* mov_word_I R0 mem_lend_I *) *)
-    (* rewrite wp_sswp. *)
-    (* iApply ((mov_word _ mem_lend_I R0) with "[p_20 PCz acc tx R0z]"); iFrameAutoSolve. *)
-    (* rewrite HIn. *)
-    (* set_solver +. *)
-    (* set_solver +. *)
-    (* rewrite HIn. *)
-    (* assumption. *)
-    (* set_solver +. *)
-    (* iModIntro. *)
-    (* iIntros "(PCz & _ & acc & tx & R0z) _". *)
-    (* (* mov_word_I R1 mem_descriptor_length *) *)
-    (* rewrite wp_sswp. *)
-    (* iApply ((mov_word _ mem_descriptor_length R1) with "[p_21 PCz acc tx R1z]"); iFrameAutoSolve. *)
-    (* rewrite HIn. *)
-    (* set_solver +. *)
-    (* set_solver +. *)
-    (* rewrite HIn. *)
-    (* assumption. *)
-    (* set_solver +. *)
-    (* iModIntro. *)
-    (* iIntros "(PCz & _ & acc & tx & R1z) _". *)
-    (* (* lend *) *)
-    (* rewrite wp_sswp. *)
-    (* iApply ((mem_lend (p_tx := tpa p_tx0) (wi := hvc_I) (hvcf := Lend) *)
-    (*            (sacc := ({[tpa addr]} ∪ {[p_pg0; tpa p_tx0]}))  *)
-    (*            (r0 := mem_lend_I) (r1 := mem_descriptor_length) (r2 := r2) *)
-    (*            (((((((((((((((((((((p_pg0 ^+ 1) ^+ 1) ^+ 1) ^+ 1) ^+ 1) ^+ 1) ^+ 1) ^+ 1) ^+ 1) ^+ 1) ^+ 1) ^+ 1) ^+ 1) ^+ 1) ^+ 1) ^+ 1) ^+ 1) ^+ 1) ^+ 1) ^+ 1) ^+ 1)%f *)
-    (*            V1 ({[ of_imm p_tx0 := of_imm (encode_vmid V0); *)
-    (*                           (p_tx0 ^+ 1)%f := of_imm zero; *)
-    (*                           ((p_tx0 ^+ 1) ^+ 1)%f := of_imm one; *)
-    (*                           (((p_tx0 ^+ 1) ^+ 1) ^+ 1)%f := of_imm (encode_vmid V1); *)
-    (*                           ((((p_tx0 ^+ 1) ^+ 1) ^+ 1) ^+ 1)%f := of_imm addr ]} : gmap Addr Addr) *)
-    (*            hs_all (singleton (tpa addr))) *)
-    (*          with "[p_22 PCz acc R0z R1z R2z hp tx txmem1 txmem2 txmem3 txmem4 txmem5]"). *)
-    (* { *)
-    (*   apply elem_of_union_r. *)
-    (*   apply elem_of_union_l. *)
-    (*   apply elem_of_singleton_2. *)
-    (*   rewrite HIn. *)
-    (*   reflexivity. *)
-    (*   set_solver +. *)
-    (* } *)
-    (* { *)
-    (*   rewrite HIn. *)
-    (*   assumption. *)
-    (*   set_solver +. *)
-    (* } *)
-    (* { *)
-    (*   apply decode_encode_instruction. *)
-    (* } *)
-    (* { *)
-    (*   apply decode_encode_hvc_func. *)
-    (* } *)
-    (* { *)
-    (*   reflexivity. *)
-    (* } *)
-    (* { *)
-    (*   unfold mem_descriptor_length. *)
-    (*   simpl. *)
-    (*   lia. *)
-    (* } *)
-    (* { *)
-    (*   (* clear. *) *)
-    (*   (* unfold parse_transaction_descriptor. *) *)
-    (*   (* unfold parse_list_of_Word. *) *)
-    (*   (* unfold monad.List.sequence_a_list. *) *)
-    (*   (* unfold sequence_a. *) *)
-    (*   (* unfold List.traversable_list. *) *)
-    (*   (* unfold monad.List.sequence_a_list. *) *)
-    (*   admit. *)
-    (* } *)
-    (* { *)
-    (*   auto. *)
-    (* } *)
-    (* { *)
-    (*   set_solver +. *)
-    (* } *)
-    (* { *)
-    (*   unfold hs_all. *)
-    (*   clear. *)
-    (*   apply non_empty_inhabited_L with W0. *)
-    (*   apply elem_of_union_l. *)
-    (*   apply elem_of_singleton_2. *)
-    (*   reflexivity. *)
-    (* } *)
-    (* { *)
-    (*   iFrame. *)
-    (*   iSplitR "txmem1 txmem2 txmem3 txmem4 txmem5". *)
-    (*   (* ([∗ set] p ∈ {[tpa addr]}, p -@O> V0 ∗ p -@E> true) *) *)
-    (*   admit. *)
-    (*   iNext. *)
-    (*   unfold memory_page. *)
-    (*   iSplit. *)
-    (*   - admit. (* fix descriptor *) *)
-    (*   - clear. *)
-    (*     rewrite ->4big_opM_insert; *)
-    (*       rewrite ?lookup_insert_None; *)
-    (*       rewrite ?lookup_singleton_None; *)
-    (*       rewrite ?lookup_empty. *)
-    (*     rewrite big_opM_singleton. *)
-    (*     iFrame. *)
-    (*     all: destruct p_tx0 as [[a1 a2] b];           *)
-    (*       simpl in b; *)
-    (*       unfold finz.incr_default; *)
-    (*       unfold finz.largest; *)
-    (*       simpl; *)
-    (*       intuition; *)
-    (*       try solve_finz. *)
-    (* } *)
-    (* iModIntro. *)
-    (* iIntros "(PCz & _ & OE & acc & R0z & R1z & (%wh & whin & R2z & whtans & whretri & whfresh) & tx & txmem) _". *)
-    (* assert ((({[tpa addr]} ∪ {[p_pg0; tpa p_tx0]}) ∖ {[tpa addr]}) = {[p_pg0; tpa p_tx0]}) as ->. *)
-    (* { *)
-    (*   (* tpa addr ≠ p_pg0 *) *)
-    (*   admit. *)
-    (* } *)
-    (* (* mov_word_I R5 p_tx0 *) *)
-    (* rewrite wp_sswp. *)
-    (* iApply ((mov_word _ p_tx0 R5) with "[p_23 PCz acc tx R5z]"); iFrameAutoSolve. *)
-    (* rewrite HIn. *)
-    (* set_solver +. *)
-    (* set_solver +. *)
-    (* rewrite HIn. *)
-    (* assumption. *)
-    (* set_solver +. *)
-    (* iModIntro. *)
-    (* iIntros "(PCz & _ & acc & tx & R5z) _". *)
-    (* (* str_I R2 R5 *) *)
-    (* rewrite wp_sswp.     *)
-    (* iApply ((str _ _ R2 R5) with "[p_24 PCz acc txmem RX0page tx R2z R5z]"); iFrameAutoSolve. *)
-    (* (* solvable *) *)
-    (* admit. *)
-    (* rewrite HIn. *)
-    (* assumption. *)
-    (* set_solver +. *)
-    (* assert (tpa p_tx0 ≠ p_rx0) as temp. *)
-    (* admit. *)
-    (* exact temp. *)
-    (* admit. *)
-    (* iModIntro. *)
-    (* iIntros "(PCz & _ & R5z & txmem & R2z & acc & tx & RX0page) _". *)
-    (* rewrite wp_sswp. *)
-    (* (* mov_reg_I R3 R3 *) *)
-    (* iApply ((mov_reg _ _ R3 R2) with "[p_25 PCz acc tx R2z R3z]"); iFrameAutoSolve. *)
-    (* admit. *)
-    (* rewrite HIn. *)
-    (* assumption. *)
-    (* set_solver +. *)
-    (* iModIntro. *)
-    (* iIntros "(PCz & _ & acc & tx & R3z & R2z) _". *)
-    (* (* mov_word_I R0 msg_send_I *) *)
-    (* rewrite wp_sswp. *)
-    (* iApply ((mov_word _ msg_send_I R0) with "[p_26 PCz acc tx R0z]"); iFrameAutoSolve. *)
-    (* rewrite HIn. *)
-    (* set_solver +. *)
-    (* set_solver +. *)
-    (* rewrite HIn. *)
-    (* assumption. *)
-    (* set_solver +. *)
-    (* iModIntro. *)
-    (* iIntros "(PCz & _ & acc & tx & R0z) _". *)
-    (* (* mov_word_I R1 one *) *)
-    (* rewrite wp_sswp. *)
-    (* iApply ((mov_word _ (encode_vmid V1) R1) with "[p_27 PCz acc tx R1z]"); iFrameAutoSolve. *)
-    (* rewrite HIn. *)
-    (* set_solver +. *)
-    (* set_solver +. *)
-    (* rewrite HIn. *)
-    (* assumption. *)
-    (* set_solver +. *)
-    (* iModIntro. *)
-    (* iIntros "(PCz & _ & acc & tx & R1z) _". *)
-    (* (* mov_word_I R2 one *) *)
-    (* rewrite wp_sswp. *)
-    (* iApply ((mov_word _ one R2) with "[p_28 PCz acc tx R2z]"); iFrameAutoSolve. *)
-    (* rewrite HIn. *)
-    (* set_solver +. *)
-    (* set_solver +. *)
-    (* rewrite HIn. *)
-    (* assumption. *)
-    (* set_solver +. *)
-    (* iModIntro. *)
-    (* iIntros "(PCz & _ & acc & tx & R2z) _". *)
-    (* (* send *) *)
-    (* rewrite wp_sswp. *)
-    (* iApply ((msg_send_primary _ V1) with "[p_29 PCz acc R0z R1z R2z tx txmem RX1st RX1page RX1mem]"); iFrameAutoSolve. *)
-    (* (* BP *) *)
-
-    
-    (* iDestruct (lb_update_alloc V2 {[p_pg0]} with "LB_auth") as ">[LB_auth LB2]";first done. *)
-    (* rewrite wp_sswp. *)
-    (* iApply ((run (((p_pg0 ^+ 1) ^+ 1))%f V2 (R := True%I) *)
-    (*             (R' := PC @@ V0 ->r (((p_pg0 ^+ 1) ^+ 1) ^+ 1)%f *)
-    (*                              ∗((p_pg0 ^+ 1) ^+ 1)%f ->a hvc_I ∗ V0 -@A> {[p_pg0]} ∗ TX@ V0 := p_tx0) *)
-    (*             ) with "[PCz p_3 acc tx R0z R1z R2z prop0 prop2 acc2 LB2 hp R0 R1 R2]"); try rewrite HIn //; iFrameAutoSolve. *)
-    (* { set_solver +. } *)
-    (* { set_solver +. } *)
-    (* { set_solver +. } *)
-    (* { apply decode_encode_hvc_func. } *)
-    (* { apply decode_encode_vmid. } *)
-    (* { iSplitL "prop2". *)
-    (*   iFrame. *)
-    (*   iSplitL "prop0". *)
-    (*   done. *)
-    (*   iSplitR "";last done. *)
-    (*   iNext. *)
-    (*   iIntros "((PC & addr & acc & tx & R0' & R1') & _ & prop0)". *)
-    (*   iFrame "PC addr R0' R1' acc tx". *)
-    (*   iExists {[p_pg0]}, {[p_pg2;p_tx2;p_rx2]} , ∅, None. *)
-    (*   iFrame "acc2 LB2". *)
-    (*   iSplitL "". *)
-    (*   iPureIntro. set_solver + HnIn_p. *)
-    (*   iSplitL "hp". *)
-    (*   { *)
-    (*     iExists hs_all. *)
-    (*     iSplitL "". *)
-    (*     iPureIntro. *)
-    (*     rewrite dom_empty_L union_empty_r_L //. *)
-    (*     iFrame. *)
-    (*     rewrite big_sepM_empty //. *)
-    (*   } *)
-    (*   iSplitL "". *)
-    (*   { *)
-    (*     rewrite /transaction_pagetable_entries_transferred. *)
-    (*     rewrite /base_extra.big_sepFM. *)
-    (*     rewrite map_filter_empty big_sepM_empty //. *)
-    (*   } *)
-    (*   iSplitL "". *)
-    (*   { *)
-    (*     rewrite /retrieval_entries_transferred. *)
-    (*     rewrite /base_extra.big_sepFM. *)
-    (*     rewrite map_filter_empty big_sepM_empty //. *)
-    (*   } *)
-    (*   iSplitL "". *)
-    (*   { *)
-    (*     rewrite /memory_transferred. *)
-    (*     rewrite /trans_memory_in_trans /pages_in_trans. *)
-    (*     rewrite map_filter_empty map_fold_empty. *)
-    (*     iExists ∅. *)
-    (*     iApply memory_pages_empty. *)
-    (*   } *)
-    (*   iDestruct "R2" as "(R1' & R2 & R3)". *)
-    (*   iFrame "R1' R2 R3 prop0". *)
-    (*   iSplitL "R2z"; first (iExists r2; done). *)
-    (*   iSplitL "R0 R1". *)
-    (*   { *)
-    (*     rewrite /rx_pages. *)
-    (*     rewrite /list_of_vmids. *)
-    (*     rewrite /vm_count /rywu_vmconfig. *)
-    (*     simpl. *)
-    (*     rewrite /V2. *)
-    (*     simpl. *)
-    (*     assert (({[2%fin]} ∪ ∅) = {[2%fin]}) as ->. *)
-    (*     { set_solver. } *)
-    (*     assert (({[0%fin]} ∪ {[1%fin; 2%fin]}) = ({[2%fin]} ∪ {[0%fin; 1%fin]})) as ->. *)
-    (*     { set_solver. } *)
-    (*     rewrite difference_union_distr_l_L. *)
-    (*     rewrite difference_diag_L. *)
-    (*     set p := {[0%fin; 1%fin]}. *)
-    (*     set q := {[2%fin]}. *)
-    (*     assert ((∅ ∪ p ∖ q) = p) as ->. *)
-    (*     { subst p q; set_solver. } *)
-    (*     subst p. *)
-    (*     clear q. *)
-    (*     rewrite big_sepS_union; last set_solver. *)
-    (*     iSplitL "R0". *)
-    (*     - rewrite big_sepS_singleton. *)
-    (*       iExists p_rx0. *)
-    (*       iDestruct "R0" as "(R0 & R1 & R2)". *)
-    (*       iFrame. *)
-    (*       rewrite /mailbox.rx_page. *)
-    (*       iDestruct "R1" as "(R1 & R2)". *)
-    (*       iFrame. *)
-    (*       iExists None. *)
-    (*       rewrite mailbox.rx_state_split. *)
-    (*       iDestruct "R0" as "(R0 & R0')". *)
-    (*       iFrame. *)
-    (*       done. *)
-    (*     - rewrite big_sepS_singleton. *)
-    (*       iExists p_rx1. *)
-    (*       iDestruct "R1" as "(R0 & R1 & R2)". *)
-    (*       iFrame. *)
-    (*       rewrite /mailbox.rx_page. *)
-    (*       iDestruct "R1" as "(R1 & R2)". *)
-    (*       iFrame. *)
-    (*       iExists None. *)
-    (*       rewrite mailbox.rx_state_split. *)
-    (*       iDestruct "R0" as "(R0 & R0')". *)
-    (*       iFrame. *)
-    (*       done. *)
-    (*   } *)
-    (*   iSplit. *)
-    (*   iIntros;done. *)
-    (*   iSplitL "". *)
-    (*   iIntros;done. *)
-    (*   iSplitL "". *)
-    (*   iIntros;done. *)
-    (*   { *)
-    (*     rewrite /trans_memory_in_trans /pages_in_trans. *)
-    (*     rewrite map_filter_empty map_fold_empty. *)
-    (*     iIntros "[? _]". *)
-    (*     rewrite difference_empty_L union_empty_r_L. *)
-    (*     done. *)
-    (*   } *)
-    (* } *)
-    (* iNext. *)
-    (* iIntros "((PCz & p_3 & acc & tx) & Hprop0) Hholds0". *)
-    (* iDestruct (VMProp_holds_agree with "[Hholds0 Hprop0]") as "[P' prop0]". *)
-    (* iSplitR "Hprop0". *)
-    (* 2: { iFrame "Hprop0". } *)
-    (* iSimpl. *)
-    (* iSimpl in "Hholds0". *)
-    (* done. *)
-    (* (* getting back resources *) *)
-    (* iDestruct "P'" as ">[(% & % & % & ? & ? & % & ? & ? & ? & ? & ? & ? & ? & returnreg)|False]". *)
-    (* 2: { (* V2 does not yield *) *)
-    (* iExFalso. *)
-    (* iExact "False". *)
-    (* } *)
-    (* (* mov_word_I R0 run *) *)
-    (* rewrite wp_sswp. *)
-    (* rewrite /return_reg_rx. *)
-    (* iDestruct "returnreg" as "[returnreg | returnreg]". *)
-    (* { *)
-    (*   iDestruct "returnreg" as "(R0z & R1z & R2z)". *)
-    (*   iDestruct "R0z" as "[R0z | R0z]". *)
-    (*   { *)
-    (*     iDestruct "R0z" as "(R0z & ?)". *)
-    (*     iApply ((mov_word ((((of_pid p_pg0) ^+ 1) ^+ 1)^+ 1)%f run_I R0) with "[p_4 PCz acc tx R0z]");try rewrite HIn //; iFrameAutoSolve; try set_solver +. *)
-    (*     iModIntro. *)
-    (*     iIntros "(PCz & p_4 & acc & tx & R0z) _". *)
-    (*     (* mov_word_I R1 V1 *) *)
-    (*     rewrite wp_sswp. *)
-    (*     iApply ((mov_word (((((of_pid p_pg0) ^+ 1) ^+ 1)^+ 1) ^+ 1)%f (encode_vmid V1) R1) with "[p_5 PCz acc tx R1z]"); try rewrite HIn //; iFrameAutoSolve; try set_solver +. *)
-    (*     iModIntro. *)
-    (*     iIntros "(PCz & p_5 & acc & tx & R1z) _". *)
-    (*     (* hvc_I *) *)
-    (*     rewrite wp_sswp. *)
-    (*     iApply ((run ((((((of_pid p_pg0) ^+ 1) ^+ 1)^+ 1) ^+ 1) ^+ 1)%f V1 (R := True)) *)
-    (*               with "[PCz p_6 acc tx R0z R1z prop0 prop1]"); try rewrite HIn //;iFrameAutoSolve. *)
-    (*     { set_solver +. } *)
-    (*     { set_solver +. } *)
-    (*     { set_solver +. } *)
-    (*     { apply decode_encode_hvc_func. } *)
-    (*     { apply decode_encode_vmid. } *)
-    (*     { *)
-    (*       iSplitR "prop0". *)
-    (*       - iModIntro. *)
-    (*         iFrame "prop1". *)
-    (*       - iSplitL "prop0". *)
-    (*         iFrame "prop0". *)
-    (*         iSplitR "";last done. *)
-    (*         iNext. *)
-    (*         iIntros "((PCz & p_6 & acc & tx & R0z & R1z) & _ & prop)". *)
-    (*         iFrame "R0z R1z prop". *)
-    (*         iCombine "PCz p_6 acc tx" as "R'". *)
-    (*         iExact "R'". *)
-    (*     } *)
-    (*     iModIntro. *)
-    (*     iIntros "[(PC & p_6 & acc & tx) prop0] Hholds". *)
-    (*     iDestruct (VMProp_holds_agree with "[Hholds prop0]") as "[P' prop0]". *)
-    (*     simpl. *)
-    (*     iFrame "Hholds prop0". *)
-    (*     (* getting back resources *) *)
-    (*     iDestruct "P'" as "((>R0z & >R1z) & prop1)". *)
-    (*     (* halt_I *) *)
-    (*     rewrite wp_sswp. *)
-    (*     iApply ((halt (((((((of_pid p_pg0) ^+ 1) ^+ 1) ^+ 1) ^+ 1) ^+ 1) ^+ 1)%f) with "[PC p_7 acc tx]"); *)
-    (*       try rewrite HIn //; iFrameAutoSolve;try set_solver +. *)
-    (*     iNext. *)
-    (*     iIntros "( PCz & p_7 & acc & tx)". *)
-    (*     iIntros "_". *)
-    (*     iApply wp_terminated'; eauto. *)
-    (*     assert ((((((((p_pg0 ^+ 1) ^+ 1) ^+ 1) ^+ 1) ^+ 1) ^+ 1) ^+ 1)%f = ((of_pid p_pg0) ^+ length rywu_program0)%f) as ->. *)
-    (*     { *)
-    (*       assert ( (Z.of_nat (length rywu_program0)) = 7%Z) as ->. by compute. *)
-    (*       solve_finz. *)
-    (*     } *)
-    (*     iFrame. *)
-    (*     iSplitR; first done. *)
-    (*     done. *)
-    (*   } *)
-    (*   { *)
-    (*     iDestruct "R0z" as "(R0z & ?)". *)
-    (*     iApply ((mov_word ((((of_pid p_pg0) ^+ 1) ^+ 1)^+ 1)%f run_I R0) with "[p_4 PCz acc tx R0z]");try rewrite HIn //; iFrameAutoSolve; try set_solver +. *)
-    (*     iModIntro. *)
-    (*     iIntros "(PCz & p_4 & acc & tx & R0z) _". *)
-    (*     (* mov_word_I R1 V1 *) *)
-    (*     rewrite wp_sswp. *)
-    (*     iApply ((mov_word (((((of_pid p_pg0) ^+ 1) ^+ 1)^+ 1) ^+ 1)%f (encode_vmid V1) R1) with "[p_5 PCz acc tx R1z]"); try rewrite HIn //; iFrameAutoSolve; try set_solver +. *)
-    (*     iModIntro. *)
-    (*     iIntros "(PCz & p_5 & acc & tx & R1z) _". *)
-    (*     (* hvc_I *) *)
-    (*     rewrite wp_sswp. *)
-    (*     iApply ((run ((((((of_pid p_pg0) ^+ 1) ^+ 1)^+ 1) ^+ 1) ^+ 1)%f V1 (R := True)) *)
-    (*               with "[PCz p_6 acc tx R0z R1z prop0 prop1]"); try rewrite HIn //;iFrameAutoSolve. *)
-    (*     { set_solver +. } *)
-    (*     { set_solver +. } *)
-    (*     { set_solver +. } *)
-    (*     { apply decode_encode_hvc_func. } *)
-    (*     { apply decode_encode_vmid. } *)
-    (*     { *)
-    (*       iSplitR "prop0". *)
-    (*       - iModIntro. *)
-    (*         iFrame "prop1". *)
-    (*       - iSplitL "prop0". *)
-    (*         iFrame "prop0". *)
-    (*         iSplitR "";last done. *)
-    (*         iNext. *)
-    (*         iIntros "((PCz & p_6 & acc & tx & R0z & R1z) & _ & prop)". *)
-    (*         iFrame "R0z R1z prop". *)
-    (*         iCombine "PCz p_6 acc tx" as "R'". *)
-    (*         iExact "R'". *)
-    (*     } *)
-    (*     iModIntro. *)
-    (*     iIntros "[(PC & p_6 & acc & tx) prop0] Hholds". *)
-    (*     iDestruct (VMProp_holds_agree with "[Hholds prop0]") as "[P' prop0]". *)
-    (*     simpl. *)
-    (*     iFrame "Hholds prop0". *)
-    (*     (* getting back resources *) *)
-    (*     iDestruct "P'" as "((>R0z & >R1z) & prop1)". *)
-    (*     (* halt_I *) *)
-    (*     rewrite wp_sswp. *)
-    (*     iApply ((halt (((((((of_pid p_pg0) ^+ 1) ^+ 1) ^+ 1) ^+ 1) ^+ 1) ^+ 1)%f) with "[PC p_7 acc tx]"); *)
-    (*       try rewrite HIn //; iFrameAutoSolve;try set_solver +. *)
-    (*     iNext. *)
-    (*     iIntros "( PCz & p_7 & acc & tx)". *)
-    (*     iIntros "_". *)
-    (*     iApply wp_terminated'; eauto. *)
-    (*     assert ((((((((p_pg0 ^+ 1) ^+ 1) ^+ 1) ^+ 1) ^+ 1) ^+ 1) ^+ 1)%f = ((of_pid p_pg0) ^+ length rywu_program0)%f) as ->. *)
-    (*     { *)
-    (*       assert ( (Z.of_nat (length rywu_program0)) = 7%Z) as ->. by compute. *)
-    (*       solve_finz. *)
-    (*     } *)
-    (*     iFrame. *)
-    (*     iSplitR; first done. *)
-    (*     done. *)
-    (*   }       *)
-    (* } *)
-    (* { *)
-    (*   iDestruct "returnreg" as "(R0z & ? & R1z)". *)
-    (*   iApply ((mov_word ((((of_pid p_pg0) ^+ 1) ^+ 1)^+ 1)%f run_I R0) with "[p_4 PCz acc tx R0z]");try rewrite HIn //; iFrameAutoSolve; try set_solver +. *)
-    (*   iModIntro. *)
-    (*   iIntros "(PCz & p_4 & acc & tx & R0z) _". *)
-    (*   (* mov_word_I R1 V1 *) *)
-    (*   rewrite wp_sswp. *)
-    (*   iDestruct "R1z" as "(%j & %p_rx & %l & ? & ? & ? & R1z & R2z & ?)". *)
-    (*   iDestruct "R1z" as "(%r3 & R1z & ?)". *)
-    (*   iApply ((mov_word (((((of_pid p_pg0) ^+ 1) ^+ 1)^+ 1) ^+ 1)%f (encode_vmid V1) R1) with "[p_5 PCz acc tx R1z]"); try rewrite HIn //; iFrameAutoSolve; try set_solver +. *)
-    (*   iModIntro. *)
-    (*   iIntros "(PCz & p_5 & acc & tx & R1z) _". *)
-    (*   (* hvc_I *) *)
-    (*   rewrite wp_sswp. *)
-    (*   iApply ((run ((((((of_pid p_pg0) ^+ 1) ^+ 1)^+ 1) ^+ 1) ^+ 1)%f V1 (R := True)) *)
-    (*             with "[PCz p_6 acc tx R0z R1z prop0 prop1]"); try rewrite HIn //;iFrameAutoSolve. *)
-    (*   { set_solver +. } *)
-    (*   { set_solver +. } *)
-    (*   { set_solver +. } *)
-    (*   { apply decode_encode_hvc_func. } *)
-    (*   { apply decode_encode_vmid. } *)
-    (*   { *)
-    (*     iSplitR "prop0". *)
-    (*     - iModIntro. *)
-    (*       iFrame "prop1". *)
-    (*     - iSplitL "prop0". *)
-    (*       iFrame "prop0". *)
-    (*       iSplitR "";last done. *)
-    (*       iNext. *)
-    (*       iIntros "((PCz & p_6 & acc & tx & R0z & R1z) & _ & prop)". *)
-    (*       iFrame "R0z R1z prop". *)
-    (*       iCombine "PCz p_6 acc tx" as "R'". *)
-    (*       iExact "R'". *)
-    (*   } *)
-    (*   iModIntro. *)
-    (*   iIntros "[(PC & p_6 & acc & tx) prop0] Hholds". *)
-    (*   iDestruct (VMProp_holds_agree with "[Hholds prop0]") as "[P' prop0]". *)
-    (*   simpl. *)
-    (*   iFrame "Hholds prop0". *)
-    (*   (* getting back resources *) *)
-    (*   iDestruct "P'" as "((>R0z & >R1z) & prop1)". *)
-    (*   (* halt_I *) *)
-    (*   rewrite wp_sswp. *)
-    (*   iApply ((halt (((((((of_pid p_pg0) ^+ 1) ^+ 1) ^+ 1) ^+ 1) ^+ 1) ^+ 1)%f) with "[PC p_7 acc tx]"); *)
-    (*     try rewrite HIn //; iFrameAutoSolve;try set_solver +. *)
-    (*   iNext. *)
-    (*   iIntros "( PCz & p_7 & acc & tx)". *)
-    (*   iIntros "_". *)
-    (*   iApply wp_terminated'; eauto. *)
-    (*   assert ((((((((p_pg0 ^+ 1) ^+ 1) ^+ 1) ^+ 1) ^+ 1) ^+ 1) ^+ 1)%f = ((of_pid p_pg0) ^+ length rywu_program0)%f) as ->. *)
-    (*   { *)
-    (*     assert ( (Z.of_nat (length rywu_program0)) = 7%Z) as ->. by compute. *)
-    (*     solve_finz. *)
-    (*   } *)
-    (*   iFrame. *)
-    (*   iSplitR; first done. *)
-    (*   done. *)
-    (* } *)
-  Qed.
-
-  Lemma rywu_machine1 p_pg1 p_tx1:
-    p_tx1 ≠ p_pg1 ->
-    seq_in_page (of_pid p_pg1) (length rywu_program1) p_pg1 ->
-    (program rywu_program1 (of_pid p_pg1))
-    ∗ VMProp V1 ((R0 @@ V0 ->r run_I ∗ R1 @@ V0 ->r encode_vmid V1 )
-                 ∗ VMProp V0 ((R0 @@ V0 ->r yield_I ∗ R1 @@ V0 ->r encode_vmid V1 ) ∗ VMProp V1 False%I (1/2)%Qp) (1/2)%Qp)%I (1/2)%Qp
-    ∗ PC @@ V1 ->r (of_pid p_pg1)
-    ∗ (∃ r0, R0 @@ V1 ->r r0)
-    ∗ V1 -@A> {[p_pg1]}
-    ∗ TX@ V1 := p_tx1
-    ⊢ VMProp_holds V1 (1/2)%Qp -∗
-    (WP ExecI @ V1 {{ (λ m, False)}}).
-  Proof.
-    iIntros (Hnottx HIn) "((p_1 & p_2 & _) & prop1 & PC1 & [%r0 R01] & acc & tx)".
-    iIntros "Hholds".
-    iDestruct (VMProp_holds_agree V1 with "[Hholds prop1]") as "[P prop1]".
+    (* (* mov_word_I R4 one *) *)
+    rewrite wp_sswp.
+    iEval (rewrite finz_plus_one_simpl) in "PCz".
+    rewrite Z_of_nat_simpl.
+    iEval (simpl) in "PCz".
+    iApply ((@mov_word _ _ _ _ _ _ _ _ _ ({[tpa addr]} ∪ {[p_pg0; tpa p_tx0]}) (tpa p_tx0)
+               (p_pg0 ^+ 14%nat)%f
+               (encode_vmid V1) R4) with "[p_15 PCz acc tx R4z]").
+    apply decode_encode_instruction.
+    apply elem_of_union_r.
+    apply elem_of_union_l.
+    apply elem_of_singleton_2.
+    rewrite (finz_succN_pid' p_pg0 14).
+    reflexivity.
+    lia.
+    rewrite HIn.
+    rewrite to_pid_aligned_eq.
+    assumption.
+    apply finz_succN_in_seq; simpl; lia.
+    rewrite Htxeq.
     iFrame.
-    pose proof (seq_in_page_forall2 _ _ _ HIn) as Hforall.
-    clear HIn; rename Hforall into HIn.
-    assert (1 = V1) as HV1.
-    by simpl.
-    (* mov_word_I R0 yield_I *)    
-    rewrite wp_sswp.
-    iDestruct "P" as "[(R0z & R1z) prop0]".
-    iApply ((mov.mov_word (of_pid p_pg1) yield_I R0) with "[p_1 PC1 acc tx R01]");try rewrite HIn //;iFrameAutoSolve;try set_solver.
     iModIntro.
-    iIntros "(PC1 & p_1 & acc & tx & R01)".
-    iSimpl.
-    rewrite HV1.
-    iIntros "_".
-    (* hvc_I *)
+    iIntros "(PCz & _ & acc & tx & R4z) _".
     rewrite wp_sswp.
-    iApply ((yield ((of_pid p_pg1) ^+ 1)%f True False%I)
-         with "[PC1 p_2 acc tx R01 R0z R1z prop0 prop1]"); try rewrite HIn //;iFrameAutoSolve.
-    { set_solver +. }
-    { set_solver +. }
-    { set_solver +. }
-    { apply decode_encode_hvc_func. }
-    { iSplitL "prop0".
-      iFrame.
-      iSplitL "prop1".
-      iFrame.
-      iSplitL "";last done.
+    iEval (rewrite finz_plus_one_simpl) in "PCz".
+    rewrite Z_of_nat_simpl.
+    iEval (simpl) in "PCz".
+    iApply ((@str _ _ _ _ _ _ _ (encode_vmid V1) w4 1%Qp p_rx0 (tpa p_tx0) ({[tpa addr]} ∪ {[p_pg0; tpa p_tx0]}) (p_pg0 ^+ 15%nat)%f (((p_tx0 ^+ 1) ^+ 1) ^+ 1)%f R4 R5) with "[p_16 PCz acc txmem4 RX0page tx R4z R5z]").
+    apply decode_encode_instruction.
+    apply union_subseteq_r'.
+    apply union_least.
+    rewrite singleton_subseteq_l.    
+    apply elem_of_union_r.
+    apply elem_of_singleton_2.
+    {
+      rewrite to_pid_aligned_eq.
+      repeat (rewrite finz_succN_one).
+      repeat (rewrite finz_succN_idemp).
+      simpl.
+      rewrite finz_succN_correct.
+      rewrite (finz_succN_pid' p_tx0 3).
+      reflexivity.
+      lia.
+    }
+    rewrite singleton_subseteq_l.
+    apply elem_of_union_l.
+    apply elem_of_singleton_2.
+    apply HIn.
+    apply finz_succN_in_seq; simpl; lia.
+    rewrite HIn.
+    rewrite to_pid_aligned_eq.
+    assumption.
+    apply finz_succN_in_seq; simpl; lia.
+    repeat (rewrite finz_succN_one).
+    repeat (rewrite finz_succN_idemp).
+    simpl.
+    rewrite finz_succN_correct.
+    rewrite (finz_succN_pid' p_tx0 3).
+    assumption.
+    lia.
+    rewrite Htxeq.
+    iFrame.
+    iModIntro.
+    iIntros "(PCz & _ & R5z & txmem4 & R4z & acc & tx & RX0page) _".
+    (* add_I R5 R3 *)
+    rewrite wp_sswp.
+    iEval (rewrite finz_plus_one_simpl) in "PCz".
+    rewrite Z_of_nat_simpl.
+    iEval (simpl) in "PCz".
+    iApply (@add _ _ _ _ _ _ (add_I R5 R3) (((p_tx0imm ^+ 1) ^+ 1) ^+ 1)%f one 1%Qp (tpa p_tx0)
+              (p_pg0 ^+ 16%nat)%f
+              R5 R3 ({[tpa addr]} ∪ {[p_pg0; tpa p_tx0]}) with "[p_17 PCz acc R5z R3z tx]").
+    apply decode_encode_instruction. 
+    apply elem_of_union_r.
+    apply elem_of_union_l.
+    apply elem_of_singleton_2.
+    rewrite (finz_succN_pid' p_pg0 16).
+    reflexivity.
+    lia.
+    rewrite HIn.
+    rewrite to_pid_aligned_eq.
+    assumption.
+    apply finz_succN_in_seq; simpl; lia.
+    rewrite Htxeq.
+    iFrame.
+    iModIntro.
+    iIntros "(PCz & _ & R5z & R3z & acc & tx) _".
+    (* (* mov_word_I R4 one *) *)
+    rewrite wp_sswp.
+    iEval (rewrite finz_plus_one_simpl) in "PCz".
+    rewrite Z_of_nat_simpl.
+    iEval (simpl) in "PCz".
+    iApply ((@mov_word _ _ _ _ _ _ _ _ _ ({[tpa addr]} ∪ {[p_pg0; tpa p_tx0]}) (tpa p_tx0)
+               (p_pg0 ^+ 17%nat)%f
+               addr R4) with "[p_18 PCz acc tx R4z]").
+    apply decode_encode_instruction.
+    apply elem_of_union_r.
+    apply elem_of_union_l.
+    apply elem_of_singleton_2.
+    rewrite (finz_succN_pid' p_pg0 17).
+    reflexivity.
+    lia.
+    rewrite HIn.
+    rewrite to_pid_aligned_eq.
+    assumption.
+    apply finz_succN_in_seq; simpl; lia.
+    rewrite Htxeq.
+    iFrame.
+    iModIntro.
+    iIntros "(PCz & _ & acc & tx & R4z) _".
+    rewrite wp_sswp.
+    iEval (rewrite finz_plus_one_simpl) in "PCz".
+    rewrite Z_of_nat_simpl.
+    iEval (simpl) in "PCz".
+    iApply ((@str _ _ _ _ _ _ _ addr w5 1%Qp p_rx0 (tpa p_tx0) ({[tpa addr]} ∪ {[p_pg0; tpa p_tx0]}) (p_pg0 ^+ 18%nat)%f ((((p_tx0 ^+ 1) ^+ 1) ^+ 1) ^+ 1)%f R4 R5) with "[p_19 PCz acc txmem5 RX0page tx R4z R5z]").
+    apply decode_encode_instruction.
+    apply union_subseteq_r'.
+    apply union_least.
+    rewrite singleton_subseteq_l.    
+    apply elem_of_union_r.
+    apply elem_of_singleton_2.
+    {
+      rewrite to_pid_aligned_eq.
+      repeat (rewrite finz_succN_one).
+      repeat (rewrite finz_succN_idemp).
+      simpl.
+      rewrite finz_succN_correct.
+      rewrite (finz_succN_pid' p_tx0 4).
+      reflexivity.
+      lia.
+    }
+    rewrite singleton_subseteq_l.
+    apply elem_of_union_l.
+    apply elem_of_singleton_2.
+    apply HIn.
+    apply finz_succN_in_seq; simpl; lia.
+    rewrite HIn.
+    rewrite to_pid_aligned_eq.
+    assumption.
+    apply finz_succN_in_seq; simpl; lia.
+    repeat (rewrite finz_succN_one).
+    repeat (rewrite finz_succN_idemp).
+    simpl.
+    rewrite finz_succN_correct.
+    rewrite (finz_succN_pid' p_tx0 4).
+    assumption.
+    lia.
+    rewrite Htxeq.
+    iFrame.
+    iModIntro.
+    iIntros "(PCz & _ & R5z & txmem5 & R4z & acc & tx & RX0page) _".
+    rewrite wp_sswp.
+    iEval (rewrite finz_plus_one_simpl) in "PCz".
+    rewrite Z_of_nat_simpl.
+    iEval (simpl) in "PCz".
+    iApply ((@mov_word _ _ _ _ _ _ _ _ _ ({[tpa addr]} ∪ {[p_pg0; tpa p_tx0]}) (tpa p_tx0)
+               (p_pg0 ^+ 19%nat)%f
+               mem_share_I R0) with "[p_20 PCz acc tx R0z]").
+    apply decode_encode_instruction.
+    apply elem_of_union_r.
+    apply elem_of_union_l.
+    apply elem_of_singleton_2.
+    rewrite (finz_succN_pid' p_pg0 19).
+    reflexivity.
+    lia.
+    rewrite HIn.
+    rewrite to_pid_aligned_eq.
+    assumption.
+    apply finz_succN_in_seq; simpl; lia.
+    rewrite Htxeq.
+    iFrame.
+    iModIntro.
+    iIntros "(PCz & _ & acc & tx & R0z) _".
+    rewrite wp_sswp.
+    iEval (rewrite finz_plus_one_simpl) in "PCz".
+    rewrite Z_of_nat_simpl.
+    iEval (simpl) in "PCz".
+    iApply ((@mov_word _ _ _ _ _ _ _ _ _ ({[tpa addr]} ∪ {[p_pg0; tpa p_tx0]}) (tpa p_tx0)
+               (p_pg0 ^+ 20%nat)%f
+               mem_descriptor_length R1) with "[p_21 PCz acc tx R1z]").
+    apply decode_encode_instruction.
+    apply elem_of_union_r.
+    apply elem_of_union_l.
+    apply elem_of_singleton_2.
+    rewrite (finz_succN_pid' p_pg0 20).
+    reflexivity.
+    lia.
+    rewrite HIn.
+    rewrite to_pid_aligned_eq.
+    assumption.
+    apply finz_succN_in_seq; simpl; lia.
+    rewrite Htxeq.
+    iFrame.
+    iModIntro.
+    iIntros "(PCz & _ & acc & tx & R1z) _".
+    rewrite wp_sswp.
+    iEval (rewrite finz_plus_one_simpl) in "PCz".
+    rewrite Z_of_nat_simpl.
+    iEval (simpl) in "PCz".
+    iSpecialize ("txacc" $! (encode_vmid V0) zero one (encode_vmid V1) addr).
+    iDestruct ("txacc" with "[$txmem1 $txmem2 $txmem3 $txmem4 $txmem5]") as "txmem".
+    match goal with
+    | |- context [([∗ map] k↦y ∈ ?p, k ->a y)%I] => set q := p
+    end.
+    iApply ((mem_share (p_tx := tpa p_tx0) (wi := hvc_I) (hvcf := Share)
+               (sacc := ({[tpa addr]} ∪ {[p_pg0; tpa p_tx0]}))
+               (r0 := mem_share_I) (r1 := mem_descriptor_length) (r2 := r2)
+               (p_pg0 ^+ 21%nat)%f
+               V1 q
+               hs_all (singleton (tpa addr)))
+             with "[p_22 PCz acc R0z R1z R2z hp tx txmem OE]").
+    {
+      apply elem_of_union_r.
+      apply elem_of_union_l.
+      apply elem_of_singleton_2.
+      rewrite HIn.
+      reflexivity.
+      apply finz_succN_in_seq; simpl; lia.
+    }
+    {
+      rewrite HIn.
+      rewrite to_pid_aligned_eq.
+      assumption.
+      apply finz_succN_in_seq; simpl; lia.
+    }
+    {
+      apply decode_encode_instruction.
+    }
+    {
+      apply decode_encode_hvc_func.
+    }
+    {
+      reflexivity.
+    }
+    {
+      unfold mem_descriptor_length.
+      simpl.
+      lia.
+    }
+    {
+      unfold parse_transaction_descriptor.
+      assert (parse_list_of_Word q (tpa p_tx0) (Z.to_nat mem_descriptor_length) = Some ([of_imm (encode_vmid V0); of_imm zero; of_imm one; of_imm (encode_vmid V1); of_pid (tpa addr)] : list Addr)) as ->.
+      {
+        clear -Htxeq Haddr.
+        unfold parse_list_of_Word.
+        unfold sequence_a.
+        remember (tpa p_tx0) as A.
+        match goal with
+        | |- context G [Some ?l] => remember l as l'
+        end.
+        simpl.
+        match goal with
+        | |- context G [monad.List.sequence_a_list [?a; ?b; ?c; ?d; ?e]] => set a' := a; set b' := b; set c' := c; set d' := d; set e' := e
+        end.
+        assert (a' = Some (of_imm (encode_vmid V0))) as ->.
+        {
+          subst a'.
+          subst q.
+          rewrite HeqA.
+          clear -Htxeq.
+          rewrite lookup_insert_Some.
+          left.
+          split; last done.
+          rewrite <-Htxeq.
+          by rewrite to_pid_aligned_eq.
+        }
+        assert (b' = Some (of_imm zero)) as ->.
+        {
+          subst b'.
+          subst q.
+          rewrite HeqA.
+          clear -Htxeq.
+          rewrite lookup_insert_Some.
+          right.
+          split.
+          - rewrite to_pid_aligned_eq.
+            rewrite <-Htxeq.
+            intros contra.
+            destruct p_tx0.
+            simpl in *.
+            destruct z.
+            simpl in *.
+            assert ((z <=? 1999000)%Z = true).
+            {
+              rewrite Z.eqb_eq in align.
+              rewrite Z.rem_mod_nonneg in align; [| lia | lia].
+              rewrite Zmod_divides in align; last lia.
+              destruct align as [c align].
+              simplify_eq.
+              assert (c <? 2000 = true)%Z.
+              lia.
+              assert (1999000 = 1000 * 1999)%Z as ->.
+              lia.
+              apply Zle_imp_le_bool.
+              apply Zmult_le_compat_l; lia.
+            }
+            solve_finz.
+          - rewrite lookup_insert_Some.
+            left.
+            split; last done.
+            by rewrite to_pid_aligned_eq.
+        }
+        assert (c' = Some (of_imm one)) as ->.
+        {
+          subst c'.
+          subst q.
+          rewrite HeqA.
+          clear -Htxeq.
+          rewrite lookup_insert_Some.
+          right.
+          split.
+          - rewrite to_pid_aligned_eq.
+            rewrite <-Htxeq.
+            intros contra.
+            destruct p_tx0.
+            simpl in *.
+            destruct z.
+            simpl in *.
+            assert ((z <=? 1999000)%Z = true).
+            {
+              rewrite Z.eqb_eq in align.
+              rewrite Z.rem_mod_nonneg in align; [| lia | lia].
+              rewrite Zmod_divides in align; last lia.
+              destruct align as [c align].
+              simplify_eq.
+              assert (c <? 2000 = true)%Z.
+              lia.
+              assert (1999000 = 1000 * 1999)%Z as ->.
+              lia.
+              apply Zle_imp_le_bool.
+              apply Zmult_le_compat_l; lia.
+            }
+            solve_finz.
+          - rewrite lookup_insert_Some.
+            right.
+            split.
+            + rewrite to_pid_aligned_eq.
+              intros contra.
+              destruct p_tx0.
+              simpl in *.
+              destruct z.
+              simpl in *.
+              assert ((z <=? 1999000)%Z = true).
+              {
+                rewrite Z.eqb_eq in align.
+                rewrite Z.rem_mod_nonneg in align; [| lia | lia].
+                rewrite Zmod_divides in align; last lia.
+                destruct align as [c align].
+                simplify_eq.
+                assert (c <? 2000 = true)%Z.
+                lia.
+                assert (1999000 = 1000 * 1999)%Z as ->.
+                lia.
+                apply Zle_imp_le_bool.
+                apply Zmult_le_compat_l; lia.
+              }
+              solve_finz.
+            + rewrite lookup_insert_Some.
+              left.
+              split; last done.
+              by rewrite to_pid_aligned_eq.
+        }
+        assert (d' = Some (of_imm (encode_vmid V1))) as ->.
+        {
+          subst d'.
+          subst q.
+          rewrite HeqA.
+          clear -Htxeq.
+          rewrite lookup_insert_Some.
+          right.
+          split.
+          - rewrite to_pid_aligned_eq.
+            rewrite <-Htxeq.
+            intros contra.
+            destruct p_tx0.
+            simpl in *.
+            destruct z.
+            simpl in *.
+            assert ((z <=? 1999000)%Z = true).
+            {
+              rewrite Z.eqb_eq in align.
+              rewrite Z.rem_mod_nonneg in align; [| lia | lia].
+              rewrite Zmod_divides in align; last lia.
+              destruct align as [c align].
+              simplify_eq.
+              assert (c <? 2000 = true)%Z.
+              lia.
+              assert (1999000 = 1000 * 1999)%Z as ->.
+              lia.
+              apply Zle_imp_le_bool.
+              apply Zmult_le_compat_l; lia.
+            }
+            solve_finz.
+          - rewrite lookup_insert_Some.
+            right.
+            split.
+            + rewrite to_pid_aligned_eq.              
+              intros contra.
+              destruct p_tx0.
+              simpl in *.
+              destruct z.
+              simpl in *.
+              assert ((z <=? 1999000)%Z = true).
+              {
+                rewrite Z.eqb_eq in align.
+                rewrite Z.rem_mod_nonneg in align; [| lia | lia].
+                rewrite Zmod_divides in align; last lia.
+                destruct align as [c align].
+                simplify_eq.
+                assert (c <? 2000 = true)%Z.
+                lia.
+                assert (1999000 = 1000 * 1999)%Z as ->.
+                lia.
+                apply Zle_imp_le_bool.
+                apply Zmult_le_compat_l; lia.
+              }
+              solve_finz.
+            + rewrite lookup_insert_Some.
+              right.
+              split.
+              * rewrite to_pid_aligned_eq.
+                intros contra.
+                destruct p_tx0.
+                simpl in *.
+                destruct z.
+                simpl in *.
+                assert ((z <=? 1999000)%Z = true).
+                {
+                  rewrite Z.eqb_eq in align.
+                  rewrite Z.rem_mod_nonneg in align; [| lia | lia].
+                  rewrite Zmod_divides in align; last lia.
+                  destruct align as [c align].
+                  simplify_eq.
+                  assert (c <? 2000 = true)%Z.
+                  lia.
+                  assert (1999000 = 1000 * 1999)%Z as ->.
+                  lia.
+                  apply Zle_imp_le_bool.
+                  apply Zmult_le_compat_l; lia.
+                }
+                solve_finz.
+              * rewrite lookup_insert_Some.
+                left.
+                split; last done.
+                by rewrite to_pid_aligned_eq.
+        }
+        assert (e' = Some (of_pid (tpa addr))) as ->.
+        {
+          subst e'.
+          subst q.
+          rewrite HeqA.
+          clear -Htxeq Haddr.
+          rewrite lookup_insert_Some.
+          right.
+          split.
+          - rewrite to_pid_aligned_eq.
+            rewrite <-Htxeq.
+            intros contra.
+            destruct p_tx0.
+            simpl in *.
+            destruct z.
+            simpl in *.
+            assert ((z <=? 1999000)%Z = true).
+            {
+              rewrite Z.eqb_eq in align.
+              rewrite Z.rem_mod_nonneg in align; [| lia | lia].
+              rewrite Zmod_divides in align; last lia.
+              destruct align as [c align].
+              simplify_eq.
+              assert (c <? 2000 = true)%Z.
+              lia.
+              assert (1999000 = 1000 * 1999)%Z as ->.
+              lia.
+              apply Zle_imp_le_bool.
+              apply Zmult_le_compat_l; lia.
+            }
+            solve_finz.
+          - rewrite lookup_insert_Some.
+            right.
+            split.
+            + rewrite to_pid_aligned_eq.
+              intros contra.
+              destruct p_tx0.
+              simpl in *.
+              destruct z.
+              simpl in *.
+              assert ((z <=? 1999000)%Z = true).
+              {
+                rewrite Z.eqb_eq in align.
+                rewrite Z.rem_mod_nonneg in align; [| lia | lia].
+                rewrite Zmod_divides in align; last lia.
+                destruct align as [c align].
+                simplify_eq.
+                assert (c <? 2000 = true)%Z.
+                lia.
+                assert (1999000 = 1000 * 1999)%Z as ->.
+                lia.
+                apply Zle_imp_le_bool.
+                apply Zmult_le_compat_l; lia.
+              }
+              solve_finz.
+            + rewrite lookup_insert_Some.
+              right.
+              split.
+              * rewrite to_pid_aligned_eq.
+                intros contra.
+                destruct p_tx0.
+                simpl in *.
+                destruct z.
+                simpl in *.
+                assert ((z <=? 1999000)%Z = true).
+                {
+                  rewrite Z.eqb_eq in align.
+                  rewrite Z.rem_mod_nonneg in align; [| lia | lia].
+                  rewrite Zmod_divides in align; last lia.
+                  destruct align as [c align].
+                  simplify_eq.
+                  assert (c <? 2000 = true)%Z.
+                  lia.
+                  assert (1999000 = 1000 * 1999)%Z as ->.
+                  lia.
+                  apply Zle_imp_le_bool.
+                  apply Zmult_le_compat_l; lia.
+                }
+                solve_finz.
+              * rewrite lookup_insert_Some.
+                right.
+                split.
+                -- rewrite to_pid_aligned_eq.                   
+                   intros contra.
+                   destruct p_tx0.
+                   simpl in *.
+                   destruct z.
+                   simpl in *.
+                   assert ((z <=? 1999000)%Z = true).
+                   {
+                     rewrite Z.eqb_eq in align.
+                     rewrite Z.rem_mod_nonneg in align; [| lia | lia].
+                     rewrite Zmod_divides in align; last lia.
+                     destruct align as [c align].
+                     simplify_eq.
+                     assert (c <? 2000 = true)%Z.
+                     lia.
+                     assert (1999000 = 1000 * 1999)%Z as ->.
+                     lia.
+                     apply Zle_imp_le_bool.
+                     apply Zmult_le_compat_l; lia.
+                   }
+                   solve_finz.
+                -- rewrite lookup_insert_Some.
+                   left.
+                   split; last done.
+                   by rewrite to_pid_aligned_eq.
+        }
+        rewrite Heql'.
+        unfold monad.List.sequence_a_list.
+        simpl.
+        reflexivity.        
+      }
+      remember (tpa addr) as A.
+      cbn.
+      rewrite decode_encode_vmid.
+      rewrite decode_encode_vmid.
+      assert (Z.to_nat 1 = 1) as ->.
+      { lia. }
+      rewrite Nat.eqb_refl.
+      cbn.
+      rewrite HeqA.
+      assert (to_pid (tpa addr) = Some (tpa addr)) as ->.
+      {
+        rewrite to_of_pid.
+        reflexivity.
+      }
+      simpl.
+      rewrite union_empty_r_L.
+      reflexivity.
+    }
+    {
+      auto.
+    }
+    {
+      set_solver +.
+    }
+    {
+      unfold hs_all.
+      clear.
+      apply non_empty_inhabited_L with W0.
+      apply elem_of_union_l.
+      apply elem_of_singleton_2.
+      reflexivity.
+    }
+    {
+      iFrame.      
       iNext.
-      iIntros "((H1 & H2 & H3 & H4 & H5 & H6) & _ & H7)".
-      iFrame.
-      iCombine "H1 H2 H3 H4 H5" as "R'".
-      iExact "R'".
+      subst q.
+      iPureIntro.
+      rewrite !dom_insert_lookup_L.
+      assumption.
+      rewrite <-elem_of_dom.
+      rewrite domtxmem.
+      rewrite elem_of_list_to_set.
+      rewrite elem_of_addr_of_page_iff.
+      rewrite to_pid_aligned_eq.
+      repeat (rewrite finz_succN_one).
+      repeat (rewrite finz_succN_idemp).
+      simpl.
+      rewrite finz_succN_correct.
+      rewrite (finz_succN_pid' p_tx0 4).
+      reflexivity.
+      lia.
+      rewrite <-elem_of_dom.
+      rewrite !dom_insert_lookup_L.
+      rewrite domtxmem.
+      rewrite elem_of_list_to_set.
+      rewrite elem_of_addr_of_page_iff.
+      rewrite to_pid_aligned_eq.
+      repeat (rewrite finz_succN_one).
+      repeat (rewrite finz_succN_idemp).
+      simpl.
+      rewrite finz_succN_correct.
+      rewrite (finz_succN_pid' p_tx0 3).
+      reflexivity.
+      lia.
+      rewrite <-elem_of_dom.
+      rewrite domtxmem.
+      rewrite elem_of_list_to_set.
+      rewrite elem_of_addr_of_page_iff.
+      rewrite to_pid_aligned_eq.
+      repeat (rewrite finz_succN_one).
+      repeat (rewrite finz_succN_idemp).
+      simpl.
+      rewrite finz_succN_correct.
+      rewrite (finz_succN_pid' p_tx0 4).
+      reflexivity.
+      lia.
+      rewrite <-elem_of_dom.
+      rewrite !dom_insert_lookup_L.
+      rewrite domtxmem.
+      rewrite elem_of_list_to_set.
+      rewrite elem_of_addr_of_page_iff.
+      rewrite to_pid_aligned_eq.
+      repeat (rewrite finz_succN_one).
+      repeat (rewrite finz_succN_idemp).
+      simpl.
+      rewrite finz_succN_correct.
+      rewrite (finz_succN_pid' p_tx0 2).
+      reflexivity.
+      lia.
+      rewrite <-elem_of_dom.
+      rewrite domtxmem.
+      rewrite elem_of_list_to_set.
+      rewrite elem_of_addr_of_page_iff.
+      rewrite to_pid_aligned_eq.
+      repeat (rewrite finz_succN_one).
+      repeat (rewrite finz_succN_idemp).
+      simpl.
+      rewrite finz_succN_correct.
+      rewrite (finz_succN_pid' p_tx0 4).
+      reflexivity.
+      lia.
+      rewrite <-elem_of_dom.
+      rewrite !dom_insert_lookup_L.
+      rewrite domtxmem.
+      rewrite elem_of_list_to_set.
+      rewrite elem_of_addr_of_page_iff.
+      rewrite to_pid_aligned_eq.
+      repeat (rewrite finz_succN_one).
+      repeat (rewrite finz_succN_idemp).
+      simpl.
+      rewrite finz_succN_correct.
+      rewrite (finz_succN_pid' p_tx0 3).
+      reflexivity.
+      lia.
+      rewrite <-elem_of_dom.
+      rewrite domtxmem.
+      rewrite elem_of_list_to_set.
+      rewrite elem_of_addr_of_page_iff.
+      rewrite to_pid_aligned_eq.
+      repeat (rewrite finz_succN_one).
+      repeat (rewrite finz_succN_idemp).
+      simpl.
+      rewrite finz_succN_correct.
+      rewrite (finz_succN_pid' p_tx0 4).
+      reflexivity.
+      lia.
+      rewrite <-elem_of_dom.
+      rewrite !dom_insert_lookup_L.
+      rewrite domtxmem.
+      rewrite elem_of_list_to_set.
+      rewrite elem_of_addr_of_page_iff.
+      rewrite to_pid_aligned_eq.
+      repeat (rewrite finz_succN_one).
+      repeat (rewrite finz_succN_idemp).
+      simpl.
+      rewrite finz_succN_correct.
+      rewrite (finz_succN_pid' p_tx0 1).
+      reflexivity.
+      lia.
+      rewrite <-elem_of_dom.
+      rewrite domtxmem.
+      rewrite elem_of_list_to_set.
+      rewrite elem_of_addr_of_page_iff.
+      rewrite to_pid_aligned_eq.
+      repeat (rewrite finz_succN_one).
+      repeat (rewrite finz_succN_idemp).
+      simpl.
+      rewrite finz_succN_correct.
+      rewrite (finz_succN_pid' p_tx0 4).
+      reflexivity.
+      lia.
+      rewrite <-elem_of_dom.
+      rewrite !dom_insert_lookup_L.
+      rewrite domtxmem.
+      rewrite elem_of_list_to_set.
+      rewrite elem_of_addr_of_page_iff.
+      rewrite to_pid_aligned_eq.
+      repeat (rewrite finz_succN_one).
+      repeat (rewrite finz_succN_idemp).
+      simpl.
+      rewrite finz_succN_correct.
+      rewrite (finz_succN_pid' p_tx0 3).
+      reflexivity.
+      lia.
+      rewrite <-elem_of_dom.
+      rewrite domtxmem.
+      rewrite elem_of_list_to_set.
+      rewrite elem_of_addr_of_page_iff.
+      rewrite to_pid_aligned_eq.
+      repeat (rewrite finz_succN_one).
+      repeat (rewrite finz_succN_idemp).
+      simpl.
+      rewrite finz_succN_correct.
+      rewrite (finz_succN_pid' p_tx0 4).
+      reflexivity.
+      lia.
+      rewrite <-elem_of_dom.
+      rewrite !dom_insert_lookup_L.
+      rewrite domtxmem.
+      rewrite elem_of_list_to_set.
+      rewrite elem_of_addr_of_page_iff.
+      rewrite to_pid_aligned_eq.
+      repeat (rewrite finz_succN_one).
+      repeat (rewrite finz_succN_idemp).
+      simpl.
+      rewrite finz_succN_correct.
+      rewrite (finz_succN_pid' p_tx0 2).
+      reflexivity.
+      lia.
+      rewrite <-elem_of_dom.      
+      rewrite domtxmem.
+      rewrite elem_of_list_to_set.
+      rewrite elem_of_addr_of_page_iff.
+      rewrite to_pid_aligned_eq.
+      repeat (rewrite finz_succN_one).
+      repeat (rewrite finz_succN_idemp).
+      simpl.
+      rewrite finz_succN_correct.
+      rewrite (finz_succN_pid' p_tx0 4).
+      reflexivity.
+      lia.
+      rewrite <-elem_of_dom.
+      rewrite !dom_insert_lookup_L.
+      rewrite domtxmem.
+      rewrite elem_of_list_to_set.
+      rewrite elem_of_addr_of_page_iff.
+      rewrite to_pid_aligned_eq.
+      repeat (rewrite finz_succN_one).
+      repeat (rewrite finz_succN_idemp).
+      simpl.
+      rewrite finz_succN_correct.
+      rewrite (finz_succN_pid' p_tx0 3).
+      reflexivity.
+      lia.
+      rewrite <-elem_of_dom.
+      rewrite domtxmem.
+      rewrite elem_of_list_to_set.
+      rewrite elem_of_addr_of_page_iff.
+      rewrite to_pid_aligned_eq.
+      repeat (rewrite finz_succN_one).
+      repeat (rewrite finz_succN_idemp).
+      simpl.
+      rewrite finz_succN_correct.
+      rewrite (finz_succN_pid' p_tx0 4).
+      reflexivity.
+      lia.
+      rewrite <-elem_of_dom.
+      rewrite !dom_insert_lookup_L.
+      rewrite domtxmem.
+      rewrite elem_of_list_to_set.
+      rewrite elem_of_addr_of_page_iff.
+      rewrite to_pid_aligned_eq.
+      repeat (rewrite finz_succN_one).
+      repeat (rewrite finz_succN_idemp).
+      simpl.
+      rewrite <-Htxeq.
+      rewrite to_pid_aligned_eq.
+      reflexivity.
+      rewrite <-elem_of_dom.
+      rewrite domtxmem.
+      rewrite elem_of_list_to_set.
+      rewrite elem_of_addr_of_page_iff.
+      rewrite to_pid_aligned_eq.
+      repeat (rewrite finz_succN_one).
+      repeat (rewrite finz_succN_idemp).
+      simpl.
+      rewrite finz_succN_correct.
+      rewrite (finz_succN_pid' p_tx0 4).
+      reflexivity.
+      lia.
+      rewrite <-elem_of_dom.
+      rewrite !dom_insert_lookup_L.
+      rewrite domtxmem.
+      rewrite elem_of_list_to_set.
+      rewrite elem_of_addr_of_page_iff.
+      rewrite to_pid_aligned_eq.
+      repeat (rewrite finz_succN_one).
+      repeat (rewrite finz_succN_idemp).
+      simpl.
+      rewrite finz_succN_correct.
+      rewrite (finz_succN_pid' p_tx0 3).
+      reflexivity.
+      lia.
+      rewrite <-elem_of_dom.
+      rewrite domtxmem.
+      rewrite elem_of_list_to_set.
+      rewrite elem_of_addr_of_page_iff.
+      rewrite to_pid_aligned_eq.
+      repeat (rewrite finz_succN_one).
+      repeat (rewrite finz_succN_idemp).
+      simpl.
+      rewrite finz_succN_correct.
+      rewrite (finz_succN_pid' p_tx0 4).
+      reflexivity.
+      lia.
+      rewrite <-elem_of_dom.
+      rewrite !dom_insert_lookup_L.
+      rewrite domtxmem.
+      rewrite elem_of_list_to_set.
+      rewrite elem_of_addr_of_page_iff.
+      rewrite to_pid_aligned_eq.
+      repeat (rewrite finz_succN_one).
+      repeat (rewrite finz_succN_idemp).
+      simpl.
+      rewrite finz_succN_correct.
+      rewrite (finz_succN_pid' p_tx0 2).
+      reflexivity.
+      lia.
+      rewrite <-elem_of_dom.
+      rewrite domtxmem.
+      rewrite elem_of_list_to_set.
+      rewrite elem_of_addr_of_page_iff.
+      rewrite to_pid_aligned_eq.
+      repeat (rewrite finz_succN_one).
+      repeat (rewrite finz_succN_idemp).
+      simpl.
+      rewrite finz_succN_correct.
+      rewrite (finz_succN_pid' p_tx0 4).
+      reflexivity.
+      lia.
+      rewrite <-elem_of_dom.
+      rewrite !dom_insert_lookup_L.
+      rewrite domtxmem.
+      rewrite elem_of_list_to_set.
+      rewrite elem_of_addr_of_page_iff.
+      rewrite to_pid_aligned_eq.
+      repeat (rewrite finz_succN_one).
+      repeat (rewrite finz_succN_idemp).
+      simpl.
+      rewrite finz_succN_correct.
+      rewrite (finz_succN_pid' p_tx0 3).
+      reflexivity.
+      lia.
+      rewrite <-elem_of_dom.      
+      rewrite domtxmem.
+      rewrite elem_of_list_to_set.
+      rewrite elem_of_addr_of_page_iff.
+      rewrite to_pid_aligned_eq.
+      repeat (rewrite finz_succN_one).
+      repeat (rewrite finz_succN_idemp).
+      simpl.
+      rewrite finz_succN_correct.
+      rewrite (finz_succN_pid' p_tx0 4).
+      reflexivity.
+      lia.
+      rewrite <-elem_of_dom.
+      rewrite !dom_insert_lookup_L.
+      rewrite domtxmem.
+      rewrite elem_of_list_to_set.
+      rewrite elem_of_addr_of_page_iff.
+      rewrite to_pid_aligned_eq.
+      repeat (rewrite finz_succN_one).
+      repeat (rewrite finz_succN_idemp).
+      simpl.
+      rewrite finz_succN_correct.
+      rewrite (finz_succN_pid' p_tx0 1).
+      reflexivity.
+      lia.
+      rewrite <-elem_of_dom.
+      rewrite domtxmem.
+      rewrite elem_of_list_to_set.
+      rewrite elem_of_addr_of_page_iff.
+      rewrite to_pid_aligned_eq.
+      repeat (rewrite finz_succN_one).
+      repeat (rewrite finz_succN_idemp).
+      simpl.
+      rewrite finz_succN_correct.
+      rewrite (finz_succN_pid' p_tx0 4).
+      reflexivity.
+      lia.
+      rewrite <-elem_of_dom.
+      rewrite !dom_insert_lookup_L.
+      rewrite domtxmem.
+      rewrite elem_of_list_to_set.
+      rewrite elem_of_addr_of_page_iff.
+      rewrite to_pid_aligned_eq.
+      repeat (rewrite finz_succN_one).
+      repeat (rewrite finz_succN_idemp).
+      simpl.
+      rewrite finz_succN_correct.
+      rewrite (finz_succN_pid' p_tx0 3).
+      reflexivity.
+      lia.
+      rewrite <-elem_of_dom.      
+      rewrite domtxmem.
+      rewrite elem_of_list_to_set.
+      rewrite elem_of_addr_of_page_iff.
+      rewrite to_pid_aligned_eq.
+      repeat (rewrite finz_succN_one).
+      repeat (rewrite finz_succN_idemp).
+      simpl.
+      rewrite finz_succN_correct.
+      rewrite (finz_succN_pid' p_tx0 4).
+      reflexivity.
+      lia.
+      rewrite <-elem_of_dom.
+      rewrite !dom_insert_lookup_L.
+      rewrite domtxmem.
+      rewrite elem_of_list_to_set.
+      rewrite elem_of_addr_of_page_iff.
+      rewrite to_pid_aligned_eq.
+      repeat (rewrite finz_succN_one).
+      repeat (rewrite finz_succN_idemp).
+      simpl.
+      rewrite finz_succN_correct.
+      rewrite (finz_succN_pid' p_tx0 2).
+      reflexivity.
+      lia.
+      rewrite <-elem_of_dom.
+      rewrite domtxmem.
+      rewrite elem_of_list_to_set.
+      rewrite elem_of_addr_of_page_iff.
+      rewrite to_pid_aligned_eq.
+      repeat (rewrite finz_succN_one).
+      repeat (rewrite finz_succN_idemp).
+      simpl.
+      rewrite finz_succN_correct.
+      rewrite (finz_succN_pid' p_tx0 4).
+      reflexivity.
+      lia.
+      rewrite <-elem_of_dom.
+      rewrite !dom_insert_lookup_L.
+      rewrite domtxmem.
+      rewrite elem_of_list_to_set.
+      rewrite elem_of_addr_of_page_iff.
+      rewrite to_pid_aligned_eq.
+      repeat (rewrite finz_succN_one).
+      repeat (rewrite finz_succN_idemp).
+      simpl.
+      rewrite finz_succN_correct.
+      rewrite (finz_succN_pid' p_tx0 3).
+      reflexivity.
+      lia.
+      rewrite <-elem_of_dom.
+      rewrite domtxmem.
+      rewrite elem_of_list_to_set.
+      rewrite elem_of_addr_of_page_iff.
+      rewrite to_pid_aligned_eq.
+      repeat (rewrite finz_succN_one).
+      repeat (rewrite finz_succN_idemp).
+      simpl.
+      rewrite finz_succN_correct.
+      rewrite (finz_succN_pid' p_tx0 4).
+      reflexivity.
+      lia.
     }
     iModIntro.
-    iIntros "[? prop1] Hholds".
-    simpl.
-    iDestruct (VMProp_holds_agree V1 with "[prop1 Hholds]") as "[P prop1]".
+    iIntros "(PCz & _ & OE & acc & R0z & R1z & (%wh & whin & R2z & whtans & whretri & whfresh) & tx & txmem) _".
+    (* assert ((({[tpa addr]} ∪ {[p_pg0; tpa p_tx0]}) ∖ {[tpa addr]}) = {[p_pg0; tpa p_tx0]}) as ->. *)
+    (* { *)
+    (*   rewrite difference_union_distr_l_L. *)
+    (*   rewrite difference_diag_L. *)
+    (*   rewrite union_empty_l_L. *)
+    (*   rewrite difference_disjoint_L. *)
+    (*   reflexivity. *)
+    (*   rewrite disjoint_singleton_r. *)
+    (*   apply not_elem_of_union. *)
+    (*   split. *)
+    (*   - apply not_elem_of_singleton_2. *)
+    (*     assumption. *)
+    (*   - apply not_elem_of_singleton_2. *)
+    (*     rewrite to_pid_aligned_eq. *)
+    (*     assumption. *)
+    (* }  *)
+    (* mov_word_I R5 p_tx0 *)
+    rewrite wp_sswp.    
+    iEval (rewrite finz_plus_one_simpl) in "PCz".
+    rewrite Z_of_nat_simpl.
+    iEval (simpl) in "PCz".
+    iApply ((@mov_word _ _ _ _ _ _ _ _ _ ({[tpa addr]} ∪ {[p_pg0; tpa p_tx0]}) (tpa p_tx0) (p_pg0 ^+ 22%nat)%f p_tx0imm R5) with "[p_23 PCz acc tx R5z]").
+    apply decode_encode_instruction.
+    apply elem_of_union_r.
+    apply elem_of_union_l.
+    apply elem_of_singleton_2.
+    rewrite HIn.
+    reflexivity.
+    apply finz_succN_in_seq; simpl; lia.
+    rewrite HIn.
+    rewrite to_pid_aligned_eq.
+    assumption.
+    apply finz_succN_in_seq; simpl; lia.
     iFrame.
-    iMod "P".
-    by iExFalso.
-  Qed.
+    iModIntro.
+    iIntros "(PCz & _ & acc & tx & R5z) _".
+    (* str_I R2 R5 *)
+    rewrite wp_sswp.
+    iEval (rewrite finz_plus_one_simpl) in "PCz".
+    rewrite Z_of_nat_simpl.
+    iEval (simpl) in "PCz".
+    iEval (unfold memory_page) in "txmem".
+    iDestruct "txmem" as "(%domtxmem' & txmem)".
+    (* Set *)
+    iDestruct (@mem_big_sepM_split_upd _ q p_tx0imm (encode_vmid V0) with "txmem") as "txmem".
+    {
+      subst q.
+      rewrite lookup_insert_Some.
+      left.
+      split; reflexivity.
+    }
+    iDestruct "txmem" as "(txmem1 & txacc)".    
+    iApply ((@str _ _ _ _ _ _ _ wh (encode_vmid V0) 1%Qp p_rx0 (tpa p_tx0) ({[tpa addr]} ∪ {[p_pg0; tpa p_tx0]}) (p_pg0 ^+ 23%nat)%f p_tx0imm R2 R5) with "[p_24 PCz acc txmem1 RX0page tx R2z R5z]").
+    apply decode_encode_instruction.
+    apply union_subseteq_r'.
+    apply union_least.
+    rewrite singleton_subseteq_l.    
+    apply elem_of_union_r.
+    apply elem_of_singleton_2.
+    {
+      rewrite <-Htxeq.
+      rewrite to_pid_aligned_eq.
+      reflexivity.
+    }
+    rewrite singleton_subseteq_l.
+    apply elem_of_union_l.
+    apply elem_of_singleton_2.
+    apply HIn.
+    apply finz_succN_in_seq; simpl; lia.
+    rewrite HIn.
+    rewrite to_pid_aligned_eq.
+    assumption.
+    apply finz_succN_in_seq; simpl; lia.
+    rewrite <-Htxeq.
+    rewrite to_pid_aligned_eq.
+    assumption.
+    iFrame.
+    iModIntro.
+    iIntros "(PCz & _ & R5z & txmem1 & R2z & acc & tx & RX0page) _".
+    rewrite wp_sswp.
+    iEval (rewrite finz_plus_one_simpl) in "PCz".
+    rewrite Z_of_nat_simpl.
+    iEval (simpl) in "PCz".
+    iSpecialize ("txacc" $! wh).
+    iDestruct ("txacc" with "[$txmem1]") as "txmem".
+    iApply ((@mov_reg _ _ _ _ _ _ _ wh 1%Qp ({[tpa addr]} ∪ {[p_pg0; tpa p_tx0]}) (tpa p_tx0) (p_pg0 ^+ 24%nat)%f one R3 R2) with "[PCz p_25 acc tx R2z R3z]").
+    apply decode_encode_instruction.
+    apply elem_of_union_r.
+    apply elem_of_union_l.
+    apply elem_of_singleton_2.
+    apply HIn.
+    apply finz_succN_in_seq; simpl; lia.
+    rewrite HIn.
+    rewrite to_pid_aligned_eq.
+    assumption.
+    apply finz_succN_in_seq; simpl; lia.
+    iFrame.
+    iModIntro.
+    iIntros "(PCz & _ & acc & tx & R3z & R2z) _".
+    rewrite wp_sswp.
+    iEval (rewrite finz_plus_one_simpl) in "PCz".
+    rewrite Z_of_nat_simpl.
+    iEval (simpl) in "PCz".
+    iApply ((@mov_word _ _ _ _ _ _ _ _ _ ({[tpa addr]} ∪ {[p_pg0; tpa p_tx0]}) (tpa p_tx0) (p_pg0 ^+ 25%nat)%f msg_send_I R0) with "[p_26 PCz acc tx R0z]").
+    apply decode_encode_instruction.
+    apply elem_of_union_r.
+    apply elem_of_union_l.
+    apply elem_of_singleton_2.
+    rewrite HIn.
+    reflexivity.
+    apply finz_succN_in_seq; simpl; lia.
+    rewrite HIn.
+    rewrite to_pid_aligned_eq.
+    assumption.
+    apply finz_succN_in_seq; simpl; lia.
+    iFrame.
+    iModIntro.
+    iIntros "(PCz & _ & acc & tx & R0z) _".
+    rewrite wp_sswp.
+    iEval (rewrite finz_plus_one_simpl) in "PCz".
+    rewrite Z_of_nat_simpl.
+    iEval (simpl) in "PCz".
+    iApply ((@mov_word _ _ _ _ _ _ _ _ _ ({[tpa addr]} ∪ {[p_pg0; tpa p_tx0]}) (tpa p_tx0) (p_pg0 ^+ 26%nat)%f (encode_vmid V1) R1) with "[p_27 PCz acc tx R1z]").
+    apply decode_encode_instruction.
+    apply elem_of_union_r.
+    apply elem_of_union_l.
+    apply elem_of_singleton_2.
+    rewrite HIn.
+    reflexivity.
+    apply finz_succN_in_seq; simpl; lia.
+    rewrite HIn.
+    rewrite to_pid_aligned_eq.
+    assumption.
+    apply finz_succN_in_seq; simpl; lia.
+    iFrame.
+    iModIntro.
+    iIntros "(PCz & _ & acc & tx & R1z) _".
+    rewrite wp_sswp.
+    iEval (rewrite finz_plus_one_simpl) in "PCz".
+    rewrite Z_of_nat_simpl.
+    iEval (simpl) in "PCz".
+    iApply ((@mov_word _ _ _ _ _ _ _ _ _ ({[tpa addr]} ∪ {[p_pg0; tpa p_tx0]}) (tpa p_tx0) (p_pg0 ^+ 27%nat)%f one R2) with "[p_28 PCz acc tx R2z]").
+    apply decode_encode_instruction.
+    apply elem_of_union_r.
+    apply elem_of_union_l.
+    apply elem_of_singleton_2.
+    rewrite HIn.
+    reflexivity.
+    apply finz_succN_in_seq; simpl; lia.
+    rewrite HIn.
+    rewrite to_pid_aligned_eq.
+    assumption.
+    apply finz_succN_in_seq; simpl; lia.
+    iFrame.
+    iModIntro.
+    iIntros "(PCz & _ & acc & tx & R2z) _".
+    rewrite wp_sswp.
+    iEval (rewrite finz_plus_one_simpl) in "PCz".
+    rewrite Z_of_nat_simpl.
+    iEval (simpl) in "PCz".
+    iDestruct "RX1mem" as "(%rxmem & rxmem)".
+    match goal with
+    | |- context [([∗ map] k↦y ∈ ?p, k ->a y)%I] => set q' := p
+    end.
+    iApply ((@msg_send_primary _ _ _ _ _ hvc_I msg_send_I (encode_vmid V1) ({[tpa addr]} ∪ {[p_pg0; tpa p_tx0]}) (tpa p_tx0) q' 1%Qp p_rx1 rxmem one (p_pg0 ^+ 28%nat)%f V1) with "[p_29 PCz acc tx R0z R1z R2z txmem RX1st rxmem RX1page]").
+    rewrite HIn.
+    rewrite to_pid_aligned_eq.
+    assumption.
+    apply finz_succN_in_seq; simpl; lia.
+    apply elem_of_union_r.
+    apply elem_of_union_l.
+    apply elem_of_singleton_2.
+    rewrite HIn.
+    reflexivity.
+    apply finz_succN_in_seq; simpl; lia.
+    by rewrite decode_encode_instruction.
+    by rewrite decode_encode_hvc_func.
+    simpl; lia.
+    by rewrite decode_encode_vmid.
+    done.
+    iFrame.
+    iNext.
+    iPureIntro.
+    subst q'.
+    subst q.
+    rewrite dom_insert_L.
+    rewrite subseteq_union_1_L.
+    assumption.
+    apply singleton_subseteq_l.
+    apply elem_of_dom.
+    exists (encode_vmid V0).
+    apply lookup_insert.
+    iModIntro.
+    iIntros "(PCz & _ & acc & R0z & R1z & R2z & tx & RX1page & RX1st & txmem & %descr & %descrsubseteq & rxmem) _".
+    rewrite wp_sswp.
+    iEval (rewrite finz_plus_one_simpl) in "PCz".
+    rewrite Z_of_nat_simpl.
+    iEval (simpl) in "PCz".
+    iApply ((@mov_word _ _ _ _ _ _ _ _ _ ({[tpa addr]} ∪ {[p_pg0; tpa p_tx0]}) (tpa p_tx0) (p_pg0 ^+ 29%nat)%f run_I R0) with "[p_30 PCz acc tx R0z]").
+    apply decode_encode_instruction.
+    apply elem_of_union_r.
+    apply elem_of_union_l.
+    apply elem_of_singleton_2.
+    rewrite HIn.
+    reflexivity.
+    apply finz_succN_in_seq; simpl; lia.
+    rewrite HIn.
+    rewrite to_pid_aligned_eq.
+    assumption.
+    apply finz_succN_in_seq; simpl; lia.
+    iFrame.
+    iModIntro.
+    iIntros "(PCz & _ & acc & tx & R0z) _".
+    rewrite wp_sswp.
+    iEval (rewrite finz_plus_one_simpl) in "PCz".
+    rewrite Z_of_nat_simpl.
+    iEval (simpl) in "PCz".
+    iApply ((@mov_word _ _ _ _ _ _ _ _ _ ({[tpa addr]} ∪ {[p_pg0; tpa p_tx0]}) (tpa p_tx0) (p_pg0 ^+ 30%nat)%f (encode_vmid V1) R1) with "[p_31 PCz acc tx R1z]").
+    apply decode_encode_instruction.
+    apply elem_of_union_r.
+    apply elem_of_union_l.
+    apply elem_of_singleton_2.
+    rewrite HIn.
+    reflexivity.
+    apply finz_succN_in_seq; simpl; lia.
+    rewrite HIn.
+    rewrite to_pid_aligned_eq.
+    assumption.
+    apply finz_succN_in_seq; simpl; lia.
+    iFrame.
+    iModIntro.
+    iIntros "(PCz & _ & acc & tx & R1z) _".
+    rewrite wp_sswp.
+    iEval (rewrite finz_plus_one_simpl) in "PCz".
+    rewrite Z_of_nat_simpl.
+    iEval (simpl) in "PCz".
+    (* iDestruct (lb_update_alloc V1 {[p_pg0]} with "LB_auth") as ">[LB_auth LB1]";first done. *)
+    iApply ((@run _ _ _ _ _ hvc_I run_I (encode_vmid V1) 1%Qp ({[tpa addr]} ∪ {[p_pg0; tpa p_tx0]}) (tpa p_tx0) True%I True%I ((R0 @@ V0 ->r run_I ∗ R1 @@ V0 ->r encode_vmid V1) ∗ VMProp 0 ((R0 @@ V0 ->r yield_I ∗ R1 @@ V0 ->r encode_vmid V1) ∗ VMProp 1 False (1 / 2)) (1 / 2)) True%I ((R0 @@ V0 ->r yield_I ∗ R1 @@ V0 ->r encode_vmid V1) ∗ VMProp 1 False (1 / 2)) (p_pg0 ^+ 31%nat)%f V1) with "[PCz p_32 acc tx R0z R1z prop0 prop1]").
+    apply elem_of_union_r.
+    apply elem_of_union_l.
+    apply elem_of_singleton_2.
+    rewrite HIn.
+    reflexivity.
+    apply finz_succN_in_seq; simpl; lia.
+    rewrite HIn.
+    rewrite to_pid_aligned_eq.
+    assumption.
+    apply finz_succN_in_seq; simpl; lia.
+    done.
+    apply decode_encode_instruction.
+    by rewrite decode_encode_hvc_func.
+    by rewrite decode_encode_vmid.
+    iFrame "PCz p_32 acc tx R0z R1z prop0 prop1".
+    iSplit; last done.
+    iNext.
+  Abort.
 
 End proof.
